start of anchor insertion proof. progress ok. wip.

coqjit/liveness.v
@@ -113,7 +113,7 @@ Fixpoint reg_list_live
              (rl: list reg) (lv: live_abs_dr) : live_abs_dr :=
   match rl with
   | nil => lv
-  | r1 :: rs => reg_list_live rs (reg_live r1 lv)
+  | r1 :: rs => reg_live r1 (reg_list_live rs lv)
   end.
 
 (* Removing a list of live registers *)
@@ -226,7 +226,7 @@ Lemma reg_list_live_subset:
   forall rl rs, PositiveSet.Subset rs (reg_list_live rl rs).
 Proof.
   unfold PositiveSet.Subset. induction rl; intros; auto.
-  simpl. apply IHrl. apply reg_live_subset. auto.
+  simpl. apply reg_live_subset. apply IHrl. auto.
 Qed.
 
 Lemma expr_list_live_subset:
@@ -255,4 +255,441 @@ Proof.
     + destruct IHl_fs; [left | right]; simpl; try (right; auto).
       unfold not. intros [EQ | IN]; auto. 
 Qed.
+
+
+
+(** * AGREEEMENT  *)
+(* This to relate regmaps with regsets *)
+(* But IR_to_RTLBlock uses its own version of agreement *)
+
+(* Two regmaps agree on a regset iff they have the same values
+   on the registers of the regset (may be None) *)
+Definition agree (rm1 rm2:reg_map) (adr:live_abs_dr) :=
+  forall r:reg, PositiveSet.In r adr -> rm1 # r = rm2 # r.
+
+Lemma agree_refl:
+  forall rs rm,
+    agree rm rm rs.
+Proof.
+  unfold agree. intros. auto.
+Qed.
+
+Lemma agree_sym:
+  forall rs rm1 rm2,
+    agree rm1 rm2 rs ->
+    agree rm2 rm1 rs.
+Proof.
+  unfold agree. intros. symmetry. auto.
+Qed.
+
+Lemma agree_trans:
+  forall rs rm1 rm2 rm3,
+    agree rm1 rm2 rs ->
+    agree rm2 rm3 rs ->
+    agree rm1 rm3 rs.
+Proof.
+  unfold agree. intros. rewrite H; auto.
+Qed.
+
+Lemma agree_subset:
+  forall rs1 rs2 rms rmo,
+    PositiveSet.Subset rs1 rs2 ->
+    agree rms rmo rs2 ->
+    agree rms rmo rs1.
+Proof.
+  unfold agree. intros. auto.
+Qed.
+
+(* Liveness transfer preserves agree *)
+Lemma agree_transfer:
+  forall live rms rmo f pc pc' i,
+    liveness_analyze f = Some live ->
+    (ver_code f)!pc = Some i ->
+    In pc' (successors i) ->
+    agree rms rmo (live!!pc) ->
+    agree rms rmo (live_dr_transf (ver_code f) pc' (live!!pc')).
+Proof.
+  intros. apply agree_subset with (live!!pc); auto.
+  eapply liveness_successor; eauto.
+Qed.
+
+(* The following lemmas express the fact that agreeing on the regset obtained 
+   after adding registers implies agreeing on the original regset 
+   (which contains less registers) *)
+Lemma expr_live_agree:
+  forall e rs rms rmo,
+    agree rms rmo (expr_live e rs) ->
+    agree rms rmo rs.
+Proof.
+  intros. eapply agree_subset; eauto. apply expr_live_subset.
+Qed.
+
+Lemma expr_list_live_agree:
+  forall exl rs rms rmo,
+    agree rms rmo (expr_list_live exl rs) ->
+    agree rms rmo rs.
+Proof.
+  intros. eapply agree_subset; eauto. apply expr_list_live_subset.
+Qed.
+
+(* Lemma movelist_live_agree: *)
+(*   forall ml rs rms rmo, *)
+(*     agree rms rmo (movelist_live ml rs) -> *)
+(*     agree rms rmo rs. *)
+(* Proof. *)
+(*   intros. eapply agree_subset; eauto. apply movelist_subset. *)
+(* Qed. *)
+
+Lemma varmap_live_agree:
+  forall vm rs rms rmo,
+    agree rms rmo (varmap_live vm rs) ->
+    agree rms rmo rs.
+Proof.
+  intros. eapply agree_subset; eauto. apply varmap_subset.
+Qed.
+
+(* Lemma synth_live_agree: *)
+(*   forall sl rs rms rmo, *)
+(*     agree rms rmo (synth_live sl rs) -> *)
+(*     agree rms rmo rs. *)
+(* Proof. *)
+(*   intros. eapply agree_subset; eauto. apply synth_subset. *)
+(* Qed. *)
+
+Lemma agree_eval_reg:
+  forall r v rs rms rmo ,
+    agree rms rmo (reg_live r rs) ->
+    eval_reg r rms = OK v ->
+    eval_reg r rmo = OK v.
+Proof.
+  intros. unfold agree in H. unfold eval_reg in H0. rewrite H in H0.
+    2: { simpl. apply PositiveSet.add_spec. left. auto. }
+    unfold eval_reg. rewrite H0. simpl. auto.
+Qed.
+
+
+(* If two regmaps agree on the registers used for the evaluation of e, 
+   then e evaluates to the same value in both regmaps *)
+Lemma agree_eval_expr:
+  forall e v rs rms rmo ,
+    agree rms rmo (expr_live e rs) ->
+    eval_expr e rms = OK v ->
+    eval_expr e rmo = OK v.
+Proof.
+  intros. destruct e; simpl in H0.
+  - destruct (eval_reg r rms) eqn:EVALL; inv H0.
+    destruct (eval_reg r0 rms) eqn:EVALR; inv H2.
+    unfold agree in H. unfold eval_reg in EVALL. rewrite H in EVALL.
+    2: { simpl. apply PositiveSet.add_spec. left. auto. }
+    unfold eval_reg in EVALR. rewrite H in EVALR.
+    2: { simpl. apply PositiveSet.add_spec. right. apply PositiveSet.add_spec. auto. }
+    simpl. unfold eval_reg. rewrite EVALL. rewrite EVALR. simpl. auto.
+  - destruct (eval_reg r rms) eqn:EVAL; inv H0.
+    unfold agree in H. unfold eval_reg in EVAL. rewrite H in EVAL.
+    2: { simpl. apply PositiveSet.add_spec. left. auto. }
+    simpl. unfold eval_reg. rewrite EVAL. simpl. auto.
+  - destruct z. inv H0. simpl. auto.
+Qed.
+
+(* If two regmaps agree on the registers used for the evaluation of 
+   the list of expressions [le], then [le] evaluates to the same boolean value
+   in both regmaps *)
+(* Lemma agree_eval_list_expr: *)
+(*   forall rs rm1 rm2 le b, *)
+(*     agree rm1 rm2 (expr_list_live le rs) -> *)
+(*     eval_list_expr le rm1 b -> *)
+(*     eval_list_expr le rm2 b. *)
+(* Proof. *)
+(*   intros. generalize dependent b. induction le; intros; inv H0; try constructor. *)
+(*   - eapply agree_eval_expr in EVAL; eauto. *)
+(*   - eapply agree_eval_expr in EVALH; eauto. *)
+(*     econstructor; eauto. apply IHle; auto. *)
+(*     unfold agree in *. intros. apply H. simpl. *)
+(*     eapply expr_live_subset; eauto. *)
+(* Qed. *)
+
+(* If two regmaps agree on the registers used for the evaluation of 
+   the list of expressions [le], then each expression of [le] evaluates to the same value
+   in both regmaps *)
+Lemma agree_eval_list:
+  forall rs rm1 rm2 le lv,
+    agree rm1 rm2 (expr_list_live le rs) ->
+    eval_list le rm1 = OK lv ->
+    eval_list le rm2 = OK lv.
+Proof.
+  intros. generalize dependent lv.
+  induction le; intros.
+  - inv H0. simpl. auto.
+  - simpl in H0. destruct (eval_expr a rm1) eqn:EVAL1; inv H0.
+    eapply agree_eval_expr in EVAL1; eauto.
+    destruct (eval_list le rm1) eqn:EVAL2; inv H2.
+    simpl. rewrite EVAL1. simpl.
+    assert (OK l = OK l) by auto. apply IHle in H0.
+    2: { eapply agree_subset; eauto. apply expr_live_subset. }
+    rewrite H0. simpl. auto.
+Qed.
+
+Lemma agree_eval_list_reg:
+  forall rs rm1 rm2 le lv,
+    agree rm1 rm2 (reg_list_live le rs) ->
+    eval_list_reg le rm1 = OK lv ->
+    eval_list_reg le rm2 = OK lv.
+Proof.
+  intros. generalize dependent lv.
+  induction le; intros.
+  - inv H0. simpl. auto.
+  - simpl in H0. destruct (eval_reg a rm1) eqn:EVAL1; inv H0.
+    eapply agree_eval_reg in EVAL1; eauto.
+    destruct (eval_list_reg le rm1) eqn:EVAL2; inv H2.
+    simpl. rewrite EVAL1. simpl.
+    assert (OK l = OK l) by auto. apply IHle in H0.
+    2: { eapply agree_subset; eauto. simpl.
+         apply reg_live_subset. }
+    rewrite H0. simpl. auto.
+Qed.
+
+
+(* Auxiliary lemmas on movelists *)
+(* If a register is not assigned by a movelist, it contains the same value 
+   before and after the update *)
+(* Lemma not_use_movelist: *)
+(*   forall ml r rm rmu, *)
+(*     ~(In r (map fst ml)) -> *)
+(*     update_movelist ml rm rmu -> *)
+(*     rm ! r = rmu ! r. *)
+(* Proof. *)
+(*   induction ml; intros. *)
+(*   - inv H0. auto. *)
+(*   - inv H0. poseq_destr r r0. *)
+(*     + simpl in H. unfold not in H. *)
+(*       exfalso. apply H. left. auto.  *)
+(*     + rewrite PTree.gso; auto. simpl in H. *)
+(*       eapply Classical_Prop.not_or_and in H as [NEQ NIN]. apply IHml; auto. *)
+(* Qed. *)
+
+(* If a register is assigned by a movelist and two regmaps agree on all the
+   registers whose value is needed to evaluate all the expressions of
+   the movelist, then we can decompose the movelist appropriately *)
+(* Lemma reg_in_movelist: *)
+(*   forall ml r rs rm1 rm2, *)
+(*     agree rm1 rm2 (movelist_live ml rs) -> *)
+(*     In r (map fst ml) -> *)
+(*     exists ml1 ml2 e rs', *)
+(*       ml = ml1 ++ (r,e)::ml2 /\ ~(In r (map fst ml1)) /\ *)
+(*       agree rm1 rm2 (expr_live e rs'). *)
+(* Proof. *)
+(*   induction ml; intros; inv H0. *)
+(*   - simpl in H. destruct a. exists nil, ml, e, (movelist_live ml rs). *)
+(*     split; auto. *)
+(*   - simpl in H. destruct a. *)
+(*     apply IHml with r rs rm1 rm2 in H1 as [ml1 [ml2 [e' [rs' [EQ [NIN AGREE]]]]]]. *)
+(*     2: { eapply expr_live_agree. eauto. } *)
+(*     poseq_destr r r0. *)
+(*     + exists nil, (ml1 ++ (r0,e')::ml2), e, (movelist_live (ml1 ++ (r0, e') :: ml2) rs). *)
+(*       split; auto. *)
+(*     + exists ((r0,e)::ml1), ml2, e', rs'. subst. *)
+(*       split; auto; try split; auto. *)
+(*       simpl. intros [EQ' | IN]; subst; auto. *)
+(* Qed. *)
+
+(* If we assign a register [r] with a movelist, and two regmaps agree on the 
+   registers used by the expression assigned to [r], then they agree on [r]
+   after the update no matter what was the value before *)
+(* Lemma use_movelist: *)
+(*   forall ml1 ml2 ml r e rs rm1 rm1u rm2 rm2u, *)
+(*     ml = ml1 ++ (r,e)::ml2 -> *)
+(*     ~(In r (map fst ml1)) -> *)
+(*     agree rm1 rm2 (expr_live e rs) -> *)
+(*     update_movelist ml rm1 rm1u -> *)
+(*     update_movelist ml rm2 rm2u -> *)
+(*     rm1u ! r = rm2u ! r. *)
+(* Proof. *)
+(*   induction ml1. *)
+(*   - intros. inv H2; inv H4. *)
+(*     inv H3. rewrite PTree.gss. rewrite PTree.gss. f_equal. *)
+(*     eapply agree_eval_expr in EVAL; eauto. *)
+(*     eapply eval_expr_determ; eauto. *)
+(*   - intros. inv H2; inv H4. *)
+(*     inv H3. assert (r <> r0). *)
+(*     { intros contra. apply H0. simpl. left. auto. } *)
+(*     rewrite PTree.gso; auto. rewrite PTree.gso; auto. *)
+(*     eapply IHml1; eauto. intros contra. simpl in H0. *)
+(*     apply H0. right. auto. *)
+(* Qed. *)
+
+(* Two agreeing regmaps still agree after having the same update *)
+(* Lemma agree_update_movelist_aux: *)
+(*   forall ml rs rm1 rm2 rm1u rm2u, *)
+(*     agree rm1 rm2 (movelist_live ml rs) -> *)
+(*     update_movelist ml rm1 rm1u -> *)
+(*     update_movelist ml rm2 rm2u -> *)
+(*     agree rm1u rm2u (movelist_live ml rs). *)
+(* Proof. *)
+(*   induction ml; intros; inv H0; inv H1; auto. *)
+(*   unfold agree. intros. *)
+(*   simpl in H0. simpl in H. poseq_destr r r0. *)
+(*   - repeat rewrite PTree.gss. f_equal. *)
+(*     eapply agree_eval_expr in EVAL; eauto. *)
+(*     eapply eval_expr_determ; eauto. *)
+(*   - repeat (rewrite PTree.gso; auto). *)
+(*     assert (In r0 (map fst ml) \/ ~(In r0 (map fst ml))) as [IN' | NIN'] by (apply in_or_not). *)
+(*     + eapply reg_in_movelist in IN' as [ml1 [ml2 [e' [rs' [EQ [NIN'' AGREE]]]]]]; eauto. *)
+(*       * eapply use_movelist; eauto. *)
+(*       * eapply expr_live_agree; eauto. *)
+(*     + assert (rm1 ! r0 = rm' ! r0). *)
+(*       { eapply not_use_movelist; eauto. } *)
+(*       assert (rm2 ! r0 = rm'0 ! r0). *)
+(*       { eapply not_use_movelist; eauto. } *)
+(*       rewrite <- H1. rewrite <- H2. apply H. apply H0. *)
+(* Qed. *)
+
+(* Lemma agree_update_movelist: *)
+(*   forall rs rm1 rm2 rm2u ml, *)
+(*     agree rm1 rm2 (movelist_live ml rs) -> *)
+(*     update_movelist ml rm2 rm2u -> *)
+(*     exists rm1u, *)
+(*       update_movelist ml rm1 rm1u /\ *)
+(*       agree rm1u rm2u (movelist_live ml rs). *)
+(* Proof. *)
+(*   intros. generalize dependent rm2u. induction ml; intros; inv H0. *)
+(*   - exists rm1. split; auto. constructor. *)
+(*   - assert (UPDATE':= UPDATE). apply IHml in UPDATE as [rm1u [UPDATE EQ]]. *)
+(*     2: { unfold agree in *. intros. apply H. simpl. *)
+(*          apply expr_live_subset. auto. } *)
+(*     apply agree_sym in H. *)
+(*     assert (EVAL':=EVAL). *)
+(*     eapply agree_eval_expr in EVAL; eauto. *)
+(*     exists (rm1u#r<-v). split; try constructor; eauto. *)
+(*     apply agree_sym. eapply agree_update_movelist_aux; eauto; econstructor; eauto. *)
+(* Qed. *)
+
+Lemma agree_update_regmap:
+  forall rs rm1 rm2 newrm vm,
+    agree rm1 rm2 (varmap_live vm rs) ->
+    update_regmap vm rm2 = OK newrm ->
+    update_regmap vm rm1 = OK newrm.
+Proof.
+  intros. generalize dependent newrm.
+  induction vm; intros; inv H0; auto.
+  destruct a. destruct (eval_expr e rm2) eqn:EVAL1; inv H2.
+  apply agree_sym in H. eapply agree_eval_expr in EVAL1; eauto.
+  simpl. rewrite EVAL1. simpl.
+  destruct (update_regmap vm rm2) eqn:EVAL2; inv H1.
+  assert (OK r0 = OK r0) by auto. apply IHvm in H0.
+  rewrite H0. auto.
+  eapply expr_live_agree. apply agree_sym in H. simpl in H. eauto.
+Qed.
+
+(* Lemma agree_synthesize_frame: *)
+(*   forall rs rm1 rm2 p sl stack, *)
+(*     agree rm1 rm2 (synth_live sl rs) -> *)
+(*     synthesize_frame p rm2 sl stack -> *)
+(*     synthesize_frame p rm1 sl stack. *)
+(* Proof. *)
+(*   intros. generalize dependent stack. *)
+(*   induction sl; intros; inv H0; try constructor; auto. *)
+(*   - eapply agree_update_regmap in UPDATE; eauto. *)
+(*   - apply IHsl; auto. simpl in H. *)
+(*     eapply varmap_live_agree. eauto. *)
+(* Qed. *)
+
+(* It is sufficient to agree on all the registers of [rs] excepted [reg]
+   before an assignation provided we assign the same value to [reg]
+   on both sides *)
+Lemma agree_insert_dead:
+  forall rs rm rm_opt reg v,
+    agree rm rm_opt (reg_dead reg rs) ->
+    agree (rm # reg <- v) (rm_opt # reg <- v) rs.
+Proof.
+  intros. unfold agree in *.
+  intros r IN. poseq_destr r reg.
+  - rewrite PTree.gss. rewrite PTree.gss. auto.
+  - rewrite PTree.gso; auto. rewrite PTree.gso; auto. apply H.
+    apply PositiveSet.remove_spec; split; auto.
+Qed.
+
+(* updating the rm on both sides *)
+Lemma agree_insert:
+  forall rs rm rm_opt reg v,
+    agree rm rm_opt rs ->
+    agree (rm # reg <- v) (rm_opt # reg <- v) rs.
+Proof.
+  intros. apply agree_subset with (reg_dead reg rs) rs rm rm_opt in H.
+  - apply agree_insert_dead. auto.
+  - intros r IN. apply PositiveSet.remove_spec in IN as [IN _]. auto.
+Qed.
+
+(* Lemma agree_movelist_live: *)
+(*   forall ml rs rs' rms rmo, *)
+(*     agree rms rmo (movelist_live ml rs) -> *)
+(*     agree rms rmo rs -> *)
+(*     agree rms rmo rs' -> *)
+(*     agree rms rmo (movelist_live ml rs'). *)
+(* Proof. *)
+(*   induction ml; intros; auto. *)
+(*   simpl. destruct a. simpl in H. intros r' IN. *)
+(*   destruct e; destruct o; try destruct o0; simpl in *; *)
+(*     try (apply (IHml rs rs' rms rmo); assumption); poseq_destr r' r0; *)
+(*       try (apply H; apply PositiveSet.add_spec; left; reflexivity). *)
+(*   - poseq_destr r' r1. *)
+(*     + apply H. apply PositiveSet.add_spec. right. *)
+(*       apply PositiveSet.add_spec. left. auto. *)
+(*     + apply (IHml rs rs' rms rmo); auto. *)
+(*       * eapply agree_subset; try apply H. *)
+(*         intros reg IN'. repeat (apply PositiveSet.add_spec; right; auto). *)
+(*       * repeat (apply PositiveSet.add_spec in IN as [contra | IN]; auto; *)
+(*                 try contradiction). *)
+(*   - apply (IHml rs rs' rms rmo); auto. *)
+(*     + eapply agree_subset; try apply H. *)
+(*       intros reg IN'. apply PositiveSet.add_spec. right. auto. *)
+(*     + apply PositiveSet.add_spec in IN as [contra | IN]; auto. contradiction. *)
+(*   - apply (IHml rs rs' rms rmo); auto. *)
+(*     + eapply agree_subset; try apply H. *)
+(*       intros reg IN'. apply PositiveSet.add_spec. right. auto. *)
+(*     + apply PositiveSet.add_spec in IN as [contra | IN]; auto. contradiction. *)
+(*   - apply (IHml rs rs' rms rmo); auto. *)
+(*     + eapply agree_subset; try apply H. *)
+(*       intros reg IN'. apply PositiveSet.add_spec. right. auto. *)
+(*     + apply PositiveSet.add_spec in IN as [contra | IN]; auto. contradiction. *)
+(* Qed. *)
+
+(* Lemma movelist_reg_dead_subset: *)
+(*   forall ml r rs, *)
+(*     PositiveSet.Subset (movelist_dead ml (reg_dead r rs)) (reg_dead r (movelist_dead ml rs)). *)
+(* Proof. *)
+(*   induction ml; intros. *)
+(*   - simpl. intros r' IN. auto. *)
+(*   - simpl. destruct a. intros r' IN. poseq_destr r' r0. *)
+(*     + apply PositiveSet.remove_spec in IN as [_ contra]. destruct contra. auto. *)
+(*     + poseq_destr r' r. *)
+(*       * apply PositiveSet.remove_spec in IN as [IN _]. apply IHml in IN. *)
+(*         apply PositiveSet.remove_spec in IN as [_ contra]. destruct contra. auto. *)
+(*       * repeat (apply PositiveSet.remove_spec; split; auto). *)
+(*         apply PositiveSet.remove_spec in IN as [IN _]. apply IHml in IN. *)
+(*         apply PositiveSet.remove_spec in IN as [IN _]. auto. *)
+(* Qed. *)
+
+(* (* Before an update_movelist, it is sufficient to agree on all the registers *)
+(*    of [rs] excepted the registers assigned by the movelist *) *)
+(* Lemma agree_movelist_dead: *)
+(*   forall ml rs rms rmsu rmo rmou, *)
+(*     agree rms rmo (movelist_live ml (movelist_dead ml rs)) -> *)
+(*     update_movelist ml rms rmsu -> *)
+(*     update_movelist ml rmo rmou -> *)
+(*     agree rmsu rmou rs. *)
+(* Proof. *)
+(*   induction ml; intros; inv H0; inv H1; simpl in H; auto. *)
+(*   simpl in H. eapply agree_eval_expr in EVAL; eauto. *)
+(*   eapply eval_expr_determ in EVAL0; eauto. *)
+(*   inv EVAL0. apply agree_insert_dead. *)
+(*   eapply IHml; eauto. *)
+(*   apply agree_subset with *)
+(*       (movelist_live ml (reg_dead r (movelist_dead ml rs))) *)
+(*       (expr_live e (movelist_live ml (reg_dead r (movelist_dead ml rs)))) *)
+(*       rms rmo in H; try apply expr_live_subset. *)
+(*   eapply agree_movelist_live; eauto. *)
+(*   + eapply movelist_live_agree. eauto. *)
+(*   + eapply agree_subset. apply movelist_reg_dead_subset. *)
+(*     eapply movelist_live_agree. eauto. *)
+(* Qed. *)
 
