coqjit/anchor_insertion_proof.v
@@ -1,0 +1,1509 @@
+(* Verification of the Anchor Insertion pass *)
+(* The first pass of the dynamic optimizer *)
+
+Require Import IR.
+Require Import IRinterpreter.
+Require Import anchor_insertion.
+Require Import sem_properties.
+Require Import internal_simulations.
+Require Import customSmallstep.
+Require Import Coq.MSets.MSetPositive.
+Require Import Lists.SetoidList.
+Require Import def_regs.
+Require Import IRtoRTLblock_proof.
+Require Import liveness.
+Require Import monad.
+Require Import monad_impl.
+Require Import Errors.
+Require Import common.
+Require Import mixed_sem.
+Require Import assume_insertion_proof.
+
+
+Lemma Inl_In:
+  forall r l, PositiveSet.InL r l <-> In r l.
+Proof.
+  intros. induction l.
+  - split; intros. inv H. inv H.
+  - split; intros.
+    + inv H.
+      * unfold PositiveSet.E.eq in H1. subst. simpl. left. auto.
+      * apply IHl in H1. simpl. right. auto.
+    + inv H.
+      * constructor. unfold PositiveSet.E.eq. auto.
+      * apply InA_cons_tl. apply IHl. auto.
+Qed.
+
+Lemma PSin_in:
+  forall r rs,
+    PositiveSet.In r rs <-> In r (PositiveSet.elements rs).
+Proof.
+  intros. rewrite <- PositiveSet.elements_spec1.
+  apply Inl_In.
+Qed.
+
+Lemma nodup_elements:
+  forall rs, NoDup (PositiveSet.elements rs).
+Proof.
+  assert (forall l, NoDupA PositiveSet.E.eq l <-> NoDup l).
+  { intros. induction l.
+    - split; intros. constructor. constructor.
+    - split; intros.
+      + inv H. constructor.
+        * unfold not. intros. rewrite <- Inl_In in H. auto.
+        * apply IHl. auto.
+      + inv H. constructor.
+        * unfold not. intros. rewrite Inl_In in H. auto.
+        * apply IHl. auto. }
+  intros. apply H. apply PositiveSet.elements_spec2w.
+Qed.
+
+Lemma defined_ind:
+  forall a l rm,
+    NoDup (a::l) ->
+    (forall r : positive, In r (a :: l) -> (exists v : Integers.Int.int, rm ! r = Some v)) ->
+    (forall r : positive, In r l -> (exists v, (PTree.remove a rm)!r = Some v)).
+Proof.
+  intros. assert (In r (a::l)) by (right; auto). apply H0 in H2 as [v SOME].
+  exists v. rewrite PTree.gro. auto. inv H. poseq_destr r a; auto.
+Qed.
+
+Lemma eval_remove:
+  forall r1 r2 rm i,
+    eval_reg r1 (PTree.remove r2 rm) = OK i ->
+    r1 <> r2 ->
+    eval_reg r1 rm = OK i.
+Proof.
+  intros r1 r2 rm i H H0. unfold eval_reg in *.
+  rewrite PTree.gro in H; auto.
+Qed.
+
+Lemma update_more:
+  forall rm newrm l a,
+    ~ In a l ->
+    update_regmap (map (fun r : reg => (r, UNA (uplus Integers.Int.zero) r)) l) (PTree.remove a rm) = OK newrm ->
+    update_regmap (map (fun r : reg => (r, UNA (uplus Integers.Int.zero) r)) l) rm = OK newrm.
+Proof.
+  intros. generalize dependent rm. generalize dependent newrm. induction l; intros.
+  - inv H0. auto.
+  - inv H0. poseq_destr a a0.
+    + simpl in H. exfalso. apply H. left. auto.
+    + assert (~ In a l).
+      { unfold not. intros. apply H. simpl. right. auto. }
+      specialize (IHl H0). simpl. repeat ok_do.
+      unfold bind in H2. destruct (eval_reg a0 (PTree.remove a rm)) eqn:EVAL; inv H2.
+      destruct (update_regmap (map (fun r : reg => (r, UNA (uplus Integers.Int.zero) r)) l) (PTree.remove a rm)) eqn:EVAL0; inv H3.
+      apply IHl in EVAL0. rewrite EVAL0. apply eval_remove in EVAL; auto. rewrite EVAL.
+      simpl. auto.
+Qed.
+
+(* rs is a subset of the set obtained by adding successively all its elements
+   (actually both are the same set) *)
+Lemma fold_elements:
+  forall r rs,
+    PositiveSet.In r rs -> PositiveSet.In r (fold_right PositiveSet.add PositiveSet.empty (PositiveSet.elements rs)).
+Proof.
+  intros r rs. rewrite PSin_in.
+  induction (PositiveSet.elements rs).
+  - intros. inv H.
+  - simpl. intros. destruct H.
+    + apply PositiveSet.add_spec. left. auto.
+    + apply IHl in H. apply PositiveSet.add_spec. right. auto.
+Qed.
+
+(* If the regmap in the optimized version is defined on rs, the regmap obtained after 
+   deoptimizing using the identity varmap on [rs'] a subset of [rs]
+   agrees with the old regmap on rs'. *)
+Theorem defined_deopt_subset_agree:
+  forall rm rs rs' ,
+    defined rm (DefFlatRegset.Inj rs) ->
+    PositiveSet.Subset rs' rs ->
+    exists rmdeopt,
+      update_regmap (identity_varmap rs') rm = OK rmdeopt /\
+      agree rm rmdeopt rs'.
+Proof.
+  assert (forall l, NoDup l ->
+                    forall rm,
+                      (forall r, In r l -> exists v, rm!r = Some v) ->
+                      exists rmdeopt,
+                        update_regmap (map (fun r : reg => (r, UNA (uplus Integers.Int.zero) r)) l) rm = OK rmdeopt /\
+                        agree rm rmdeopt (fold_right PositiveSet.add PositiveSet.empty l)).
+  { intros l NODUP. induction l; intros.
+    - simpl in H. simpl. exists empty_regmap. split. constructor.
+      intros r IN. inv IN.
+    - specialize (defined_ind a l rm NODUP H). intros H1.
+      apply IHl in H1.
+      2: { apply NoDup_cons_iff in NODUP. destruct NODUP. auto. }
+      destruct H1 as [rmdeopt [UPDATE AGREE]].
+      assert (GETA: exists va, rm ! a = Some va).
+      { apply H. simpl. left. auto. }
+      destruct GETA as [va GETA].
+      exists (rmdeopt # a <- va). split.
+      + simpl. unfold eval_reg. rewrite GETA. simpl. apply update_more in UPDATE.
+        2: { unfold not; intros IN. inv NODUP. apply H2; auto. }
+        rewrite UPDATE. simpl. rewrite Integers.Int.add_zero. auto.
+      + unfold agree. intros r. specialize (AGREE r). poseq_destr r a.
+        * rewrite PTree.gss. auto.
+        * intros. rewrite PTree.gro in AGREE; auto. rewrite PTree.gso; auto.
+          apply PositiveSet.add_spec in H0 as [contra | IN]; auto.
+          apply HEQ in contra. inv contra. }
+  intros. specialize (H (PositiveSet.elements rs')).
+  assert (NoDup (PositiveSet.elements rs')) by (apply nodup_elements).
+  apply H with rm in H2.
+  - destruct H2 as [rmdeopt [UPDATE AGREE]]. exists rmdeopt. split; auto.
+    unfold agree. intros r IN. apply AGREE. apply fold_elements. auto.
+  - unfold defined in H0. intro. rewrite <- PSin_in. intros IN. apply H0. auto.
+Qed.
+
+Lemma deopt_subset_agree:
+  forall rm rs rs' newrm,
+    defined rm (DefFlatRegset.Inj rs) ->
+    PositiveSet.Subset rs' rs ->
+    update_regmap (identity_varmap rs') rm = OK newrm ->
+    agree rm newrm rs'.
+Proof.
+  intros. apply defined_deopt_subset_agree with rm rs rs' in H; auto.
+  destruct H as [rmdeopt [UPDATE AGREE]].
+  rewrite H1 in UPDATE. inv UPDATE. auto.
+Qed.
+
+(* If we apply update_regmap with the identity over a given regset, the 
+   resulting regmap will be undefined outside of the regset *)
+Lemma update_not_captured:
+  forall rm newrm rs r,
+    ~ PositiveSet.In r rs ->
+    update_regmap (identity_varmap rs) rm = OK newrm ->
+    newrm ! r = None.
+Proof.
+  intros rm newrm rs r. rewrite PSin_in. 
+  assert (forall l r rm newrm,
+             ~ In r l ->
+             update_regmap (map (fun r : reg => (r, UNA (uplus Integers.Int.zero) r)) l) rm = OK newrm ->
+             newrm ! r = None).
+  { induction l; intros.
+    - inv H0. unfold empty_regmap. apply PTree.gempty.
+    - inv H0. poseq_destr r0 a.
+      + simpl in H. exfalso. apply H. left. auto.
+      + destruct (eval_reg a rm0) eqn:EVAL; inv H2.
+        destruct (update_regmap (map (fun r : reg => (r, UNA (uplus Integers.Int.zero) r)) l) rm0) eqn:UPD; inv H1.
+        rewrite PTree.gso; auto. eapply IHl.
+        2: { apply UPD. }
+        intros IN. apply H. simpl. right. auto. }
+  apply H.
+Qed.
+
+(** * Properties of clean_label_list *)
+Lemma nodup_clean:
+  forall def l c,
+    NoDup (clean_label_list def c l).
+Proof.
+  intros def l c. unfold clean_label_list.
+  assert (ND: NoDup (remove_dup l)).
+  { unfold remove_dup. apply NoDup_nodup. }
+  unfold filter_unused.
+  assert (P: forall X (li:list X) f, NoDup li -> NoDup (filter f li)).
+  { intros X li f H. induction li; simpl. constructor.
+    destruct (f a) eqn:FA.
+    - constructor.
+      + unfold not. intros. apply filter_In in H0. destruct H0. inv H. apply H4. auto.
+      + apply IHli. inv H. auto.
+    - apply IHli. inv H. auto. }
+  apply P. auto.
+Qed.
+
+Definition used (l:list label) (c:code) :=
+  forall lbl, In lbl l -> exists i, c ! lbl = Some i.
+
+Lemma used_clean:
+  forall def l c, used (clean_label_list def c l) c.
+Proof.
+  unfold used. intros def l c lbl IN. unfold clean_label_list in IN.
+  apply filter_In in IN as [IN _]. apply filter_In in IN as [IN USED].
+  unfold is_used in USED. destruct (c!lbl); inv USED. eauto.
+Qed.
+
+Lemma used_cons:
+  forall a l c,
+    used (a::l) c -> used l c.
+Proof.
+  unfold used. intros a l c H lbl H0. apply H. simpl. right. auto.
+Qed.
+
+Lemma nodup_cons_in:
+  forall  (l:list label) x y,
+    NoDup (y::l) ->
+    In x (y::l) ->
+    (x = y /\ ~ In x l) \/ (x <> y /\ In x l).
+Proof.
+  intros l x y H H0. inv H. simpl in H0.
+  poseq_destr x y.
+  - left. split; auto.
+  - right. split; auto. destruct H0. exfalso. apply HEQ. auto. auto.
+Qed.
+
+
+
+(** * Matching the stack and properties  *)
+(* Matching stackframes: a version may have been replaced with its optimized version *)
+Inductive match_stackframe (v:version) (fid:fun_id) (l:list label) (live:live_abs_state) (def:def_abs_state): stackframe -> stackframe -> Prop :=
+| frame_same:              (* when doing a call from an unoptimized function *)
+    forall sf,
+      (match_stackframe v fid l live def) sf sf
+| frame_deopt:             (* when doing a call after deoptimization *)
+    forall r lbl rms rmo
+      (AGREE: forall retval, agree (rms#r<-retval) (rmo#r<-retval) (live_dr_transf (ver_code v) lbl (live_absstate_get lbl live))),
+      (match_stackframe v fid l live def) (IR_SF (r, v, lbl, rms)) (IR_SF (r, v, lbl, rmo))
+| frame_opt:               (* when doing a call from the optimized version *)
+    forall r lbl rms vins
+      (ANC_INSERT: anc_insert_version v fid l live def = OK vins)
+      (DEF: forall retval, defined (rms#r<-retval) (def_absstate_get lbl def)),
+      (match_stackframe v fid l live def) (IR_SF (r, v, lbl, rms)) (IR_SF (r, vins, lbl, rms)).
+
+(* Generalizing match_stackframe to the entire stack *)
+Inductive match_stack (v:version) (fid:fun_id) (l:list label) (live:live_abs_state) (def:def_abs_state): stack -> stack -> Prop :=
+| match_nil:
+    (match_stack v fid l live def) nil nil
+| match_cons:
+    forall s s' sf sf'
+      (MS: (match_stack v fid l live def) s s')
+      (MSF: (match_stackframe v fid l live def) sf sf'),
+      (match_stack v fid l live def) (sf::s) (sf'::s').
+
+Lemma match_stackframe_same:
+  forall v fid l live def sf,
+    (match_stackframe v fid l live def) sf sf.
+Proof.
+  intros v fid l live def sf. destruct sf; apply frame_same.
+Qed.
+
+Lemma match_stack_same:
+  forall s v fid l live def,
+    (match_stack v fid l live def) s s.
+Proof.
+  intros s v fid l live def. induction s; constructor. auto. apply match_stackframe_same.
+Qed.
+
+Lemma match_app:
+  forall synth s s' v fid l live def,
+    (match_stack v fid l live def) s s' ->
+    (match_stack v fid l live def) (synth++s) (synth++s').
+Proof.
+  intros. induction synth.
+  - simpl. auto.
+  - repeat rewrite <- app_comm_cons. apply match_cons. auto. apply match_stackframe_same.
+Qed.
+
+Lemma app_match:
+  forall synth synthopt s s' v fid l live def,
+    (match_stack v fid l live def) s s' ->
+    (match_stack v fid l live def) synth synthopt ->
+    (match_stack v fid l live def) (synth++s) (synthopt++s').
+Proof.
+  intros. induction H0.
+  - simpl. auto.
+  - repeat rewrite <- app_comm_cons. apply match_cons; auto.
+Qed.
+
+(** * Index and order used in the simulation *)
+(* There is one stuttering step for each inserted Anchor *)
+Inductive anc_index: Type :=
+| One : anc_index
+| Zero: anc_index.
+
+Inductive anc_order: anc_index -> anc_index -> Type :=
+| order: anc_order Zero One.
+
+Lemma wfounded: well_founded anc_order.
+Proof.
+  unfold well_founded. intros a. constructor. intros y H. inv H. constructor. intros y H. inv H.
+Qed.
+
+Lemma trans: Relation_Definitions.transitive _ anc_order.
+Proof.
+  unfold Relation_Definitions.transitive. intros x y z H H0. inv H. inv H0.
+Qed.
+
+(** * The match_states relation  *)
+(* This proof is a backward internal simulation.
+   Each step of the source is matched with a step of the optimized program.
+   Except for the steps of newly inserted Anchors.
+   At a new Anchor, we stutter in the source.
+
+<<
+
+       st1 --------------- st2
+        |                   |
+       t|(1 or 2 steps)     |t
+        |                   |
+        v                   v
+       st1'--------------- st2'
+
+>>
+ *)
+
+Inductive match_states (p:program) (v:version) (fid:fun_id) (lbllist:list label) (live:live_abs_state) (def:def_abs_state): anc_index -> mixed_state -> mixed_state -> Prop :=
+| anc_match:                (* matching at a new Anchor in the optimized version *)
+    forall vins s s' rms top heap lbl
+      (MATCHSTACK: (match_stack v fid lbllist live def) s s')
+      (DEF: defined rms (def_absstate_get lbl def))
+      (OPT: anc_insert_version v fid lbllist live def = OK vins)
+      (IN: In lbl lbllist),
+      (match_states p v fid lbllist live def) One
+        (Halt_IR (v, lbl, rms), mkmut s top heap)
+        (Halt_IR (vins, lbl, rms), mkmut s' top heap)
+
+| shift_match:                     (* matching at a shifted instruction *)
+    forall vins s s' rms top heap lbl fresh
+      (MATCHSTACK: (match_stack v fid lbllist live def) s s')
+      (DEF: defined rms (def_absstate_get lbl def))
+      (OPT: anc_insert_version v fid lbllist live def = OK vins)
+      (NOT_IN: ~ In fresh lbllist)
+      (SAME_CODE: (ver_code v) # lbl = (ver_code vins) # fresh),
+      (match_states p v fid lbllist live def) Zero
+        (Halt_IR (v, lbl, rms), mkmut s top heap)
+        (Halt_IR (vins, fresh, rms), mkmut s' top heap)
+
+| opt_match:                        (* matching inside the optimized version *)
+    forall vins s s' lbl rms top heap
+      (MATCHSTACK: (match_stack v fid lbllist live def) s s')
+      (DEF: defined rms (def_absstate_get lbl def))
+      (OPT: anc_insert_version v fid lbllist live def = OK vins)
+      (NOTIN: ~ In lbl lbllist),
+      (match_states p v fid lbllist live def) Zero
+        (Halt_IR (v, lbl, rms), mkmut s top heap)
+        (Halt_IR (vins, lbl, rms), mkmut s' top heap)
+
+| refl_match:                   (* matching outside of the optimized version *)
+    forall s s' synchro top heap
+      (MATCHSTACK: (match_stack v fid lbllist live def) s s'),
+      (match_states p v fid lbllist live def) Zero
+        (synchro, mkmut s top heap)
+        (synchro, mkmut s' top heap)
+
+| deopt_match:   (* matching after deoptimization at the inserted Anchors *)
+    forall s s' pc rms rmo top heap
+      (MATCHSTACK: (match_stack v fid lbllist live def) s s')
+      (AGREE: agree rms rmo (live_dr_transf (ver_code v) pc (live_absstate_get pc live))),
+      (match_states p v fid lbllist live def) Zero
+        (Halt_IR (v, pc, rms), mkmut s top heap)
+        (Halt_IR (v, pc, rmo), mkmut s' top heap).
+
+
+(** * Code preservation properties  *)
+Lemma code_preservation':        (* use at opt_match *)
+  forall vbase vins fid l_anc lbl live def,
+    anc_insert_version vbase fid l_anc live def = OK vins ->
+    ~ In lbl l_anc ->
+    forall iopt isrc,
+      (ver_code vins) # lbl = Some iopt ->
+      (ver_code vbase) # lbl = Some isrc ->
+      iopt = isrc.
+Proof.
+  intros vbase vins fid l_anc lbl live def OPT NOTIN iopt isrc CODEOPT CODESRC.
+  unfold anc_insert_version in OPT. repeat do_ok.
+  assert (H: forall cs co, insert_list_anchor (ver_code vbase) cs fid l_anc live def = OK co ->
+                           co ! lbl = Some iopt -> cs ! lbl = Some isrc -> iopt = isrc).
+  { clear HDO CODEOPT CODESRC. induction l_anc; intros.
+    - simpl in H. inv H. rewrite H0 in H1. inv H1. auto.
+    - simpl in H. repeat do_ok. simpl in NOTIN.
+      assert (NOTIN': a<>lbl /\ ~ In lbl l_anc).
+      { split; unfold not; intros; apply NOTIN. left. auto. right. auto. }
+      clear NOTIN. destruct NOTIN' as [DIFF NOTIN].
+      specialize (IHl_anc NOTIN c0 co H3 H0). unfold insert_single_anchor in HDO. repeat do_ok.
+      rewrite PTree.gso in IHl_anc; auto.
+      poseq_destr (fresh_sug (Pos.add a spacing) cs) lbl.
+      + erewrite fresh_sug_correct in H1; eauto. inv H1.
+      + rewrite PTree.gso in IHl_anc; auto. }
+  eapply H; eauto.
+Qed.
+
+Lemma code_preservation:        (* use at opt_match *)
+  forall p rtl nc p' s s' rms rmo top heap t news vbase vins fid l_anc lbl live def,
+    anc_insert_version vbase fid l_anc live def = OK vins ->
+    ~ In lbl l_anc ->
+    safe (mixed_sem p rtl nc AnchorOn) (Halt_IR (vbase, lbl, rms), mkmut s top heap) ->
+    Step (mixed_sem p' rtl nc AnchorOn) (Halt_IR (vins, lbl, rmo), mkmut s' top heap) t news ->
+    (ver_code vbase) # lbl = (ver_code vins) # lbl.
+Proof.
+  intros p rtl nc p' s s' rms rmo top heap t news vbase vins fid l_anc lbl live def H H0 H1 H2.
+  unfold safe in H1. specialize (H1 _ (star_refl _ _ _)). destruct H1 as [[r FINAL]|[t' [s'' STEP]]].
+  { inv FINAL. }
+  assert (exists iins, (ver_code vins) # lbl = Some iins).
+  { inv H2; eauto. unfold ir_step, ir_int_step in STEP0. repeat sdo_ok. eauto. }
+  assert (exists ibase, (ver_code vbase) # lbl = Some ibase).
+  { inv STEP; eauto. unfold ir_step, ir_int_step in STEP0. repeat sdo_ok. eauto. }
+  destruct H1. destruct H3. rewrite H1. rewrite H3.
+  apply f_equal. symmetry. eapply code_preservation'; eauto.
+Qed.    
+
+
+(* The pass  cannot remove any code *)
+Lemma more_code:
+  forall vbase vins fid l_anc lbl live def,
+    anc_insert_version vbase fid l_anc live def = OK vins ->
+    (ver_code vins) # lbl = None ->
+    (ver_code vbase) # lbl = None.
+Proof.
+  intros vbase vins fid l_anc lbl live def OPT CODE.
+  unfold anc_insert_version in OPT. repeat do_ok.
+  assert (H: forall cs co, insert_list_anchor (ver_code vbase) cs fid l_anc live def = OK co -> co ! lbl = None -> cs ! lbl = None).
+  { clear HDO. induction l_anc; intros.
+    - unfold insert_list_anchor in H. inv H. auto.
+    - simpl in H. repeat do_ok. specialize (IHl_anc c0 co H2 H0).
+      unfold insert_single_anchor in HDO. repeat do_ok.
+      poseq_destr a lbl.
+      + rewrite PTree.gss in IHl_anc. inv IHl_anc.
+      + rewrite PTree.gso in IHl_anc; auto.
+        poseq_destr (fresh_sug (Pos.add a spacing) cs) lbl.
+        * eapply fresh_sug_correct. eauto.
+        * rewrite PTree.gso in IHl_anc; auto. }
+  specialize (H (ver_code vbase) c HDO CODE). auto.
+Qed.
+
+Lemma more_code':
+  forall base_c cs co fid lbl anc_lbl live def,
+    insert_single_anchor base_c cs fid anc_lbl live def = OK co ->
+    co ! lbl = None ->
+    cs ! lbl = None.
+Proof.
+  intros base_c cs co fid lbl anc_lbl live def H H0. unfold insert_single_anchor in H. repeat do_ok.
+  poseq_destr anc_lbl lbl.
+  - rewrite PTree.gss in H0. inv H0.
+  - rewrite PTree.gso in H0; auto.
+    poseq_destr (fresh_sug (Pos.add anc_lbl spacing) cs) lbl.
+    + rewrite PTree.gss in H0. eapply fresh_sug_correct. eauto.
+    + rewrite PTree.gso in H0; auto.
+Qed.
+
+(* The code is preserved outside of the list of labels *)
+Lemma code_preserved:
+  forall fid lbl i l live def base_c cs co,
+    insert_list_anchor base_c cs fid l live def = OK co ->
+    cs ! lbl = Some i ->
+    ~ In lbl l ->
+    co ! lbl = Some i.
+Proof.
+  intros fid lbl i l live def base_c. induction l; intros.
+  - simpl in H. inv H. auto.
+  - simpl in H. repeat do_ok.
+    specialize (IHl c co H3). rewrite in_cns in H1. apply Decidable.not_or in H1. destruct H1.
+    apply IHl; auto.
+    unfold insert_single_anchor in HDO. repeat do_ok. rewrite PTree.gso; auto.
+    poseq_destr (fresh_sug (Pos.add a spacing) cs) lbl.
+    + erewrite fresh_sug_correct in H0; auto. inv H0.
+    + rewrite PTree.gso; auto.
+Qed.
+
+(* Used is preserved by insertion of anchor *)
+Lemma used_insert_single_anchor:
+  forall l base_c cs co fid lbl live def,
+    used l cs ->
+    insert_single_anchor base_c cs fid lbl live def = OK co ->
+    used l co.
+Proof.
+  intros. unfold insert_single_anchor in H0. repeat do_ok.
+  unfold used. intros x IN. apply H in IN as [i' CODE].
+  poseq_destr lbl x.
+  - rewrite PTree.gss. eauto.
+  - rewrite PTree.gso; auto. poseq_destr (fresh_sug (Pos.add lbl spacing) cs) x.
+    + rewrite PTree.gss. eauto.
+    + rewrite PTree.gso; auto. eauto.
+Qed.
+
+(* At the insertion point, the code is shifted *)
+Lemma code_anc:                  (* use at anc_match *)
+  forall vbase vins fid l_anc lbl live def,
+    anc_insert_version vbase fid l_anc live def = OK vins ->
+    In lbl l_anc ->
+    NoDup l_anc ->
+    used l_anc (ver_code vbase) ->
+    (exists freshlbl rs_def rs_live,
+        def_absstate_get lbl def = DefFlatRegset.Inj rs_def /\
+        live_dr_transf (ver_code vbase) lbl (live_absstate_get lbl live) = rs_live /\
+        (ver_code vins) # lbl = Some (Anchor (fid,lbl) (identity_varmap (PositiveSet.inter rs_def rs_live)) freshlbl) /\
+        (ver_code vbase) # freshlbl = None /\
+        exists i, (ver_code vbase) # lbl = Some i /\ (ver_code vins) # freshlbl = Some i).
+Proof.
+  intros vbase vins fid l_anc lbl live def OPT IN NODUP DEF.
+  unfold anc_insert_version in OPT. repeat do_ok.
+  assert (forall cs co, insert_list_anchor (ver_code vbase) cs fid l_anc live def = OK co ->
+                        In lbl l_anc -> used l_anc cs ->
+                        exists freshlbl rs_def rs_live,
+                          def_absstate_get lbl def = DefFlatRegset.Inj rs_def /\
+                          live_dr_transf (ver_code vbase) lbl (live_absstate_get lbl live) = rs_live /\
+                          co ! lbl = Some (Anchor (fid,lbl) (identity_varmap (PositiveSet.inter rs_def rs_live)) freshlbl) /\
+                          cs ! freshlbl = None /\
+                          exists i, cs ! lbl = Some i /\
+                                    co ! freshlbl = Some i).
+  { clear HDO IN. induction l_anc; intros.
+    - simpl in H. inv H. inv H0.
+    - simpl in H. repeat do_ok. apply nodup_cons_in in H0; auto.
+      destruct H0 as [[EQ NOTIN] | [DIFF IN]].
+      + subst. unfold insert_single_anchor in HDO. repeat do_ok.
+        exists (fresh_sug (Pos.add a spacing) cs). exists r.
+        exists (live_dr_transf (ver_code vbase) a (live_absstate_get a live)).
+        split; try split; auto. unfold defined_rs in HDO1. destruct (def_absstate_get a def); inv HDO1. auto. split.
+        * eapply code_preserved; eauto. rewrite PTree.gss. auto.
+        * split. { eapply fresh_sug_correct. eauto. }
+          exists i. split; auto. poseq_destr (fresh_sug (Pos.add a spacing) cs) a.
+          erewrite fresh_sug_correct in HDO; eauto. inv HDO.
+          eapply code_preserved; eauto. rewrite PTree.gso; auto. rewrite PTree.gss. auto.
+          unfold not; intro. apply used_cons in H1. apply H1 in H. destruct H.
+          erewrite fresh_sug_correct in H; auto. inv H.
+      + inv NODUP. apply used_cons in DEF as DEF'. apply used_cons in H1 as DEF''.
+        assert (used l_anc c0) by (eapply used_insert_single_anchor; eauto).
+        specialize (IHl_anc H4 DEF' c0 co H3 IN H). destruct IHl_anc as [freshlbl [rs_def [rs_live [GETDEF [GETLIVE [CO [FRESH [i [C0 CO']]]]]]]]].
+        exists freshlbl. exists rs_def. exists rs_live.
+        split; auto. split; auto. split; auto. split.
+        { eapply more_code'; eauto. }
+        exists i. split; auto.
+        unfold insert_single_anchor in HDO. repeat do_ok. rewrite PTree.gso in C0; auto.
+        poseq_destr (fresh_sug (Pos.add a spacing) cs) lbl.
+        * apply DEF'' in IN. destruct IN. erewrite fresh_sug_correct in H0; eauto. inv H0.
+        * rewrite PTree.gso in C0; auto. }
+  apply H; auto.
+Qed.
+
+Lemma code_notanc:               (* for progress preservation *)
+  forall vbase vins fid l_anc lbl live def,
+    anc_insert_version vbase fid l_anc live def = OK vins ->
+    ~ In lbl l_anc ->
+    forall i, (ver_code vbase) # lbl = Some i ->
+              (ver_code vins) # lbl = Some i.
+Proof.
+  assert (H: forall (l:list label) i lbl fid live def base_c cs co,
+             insert_list_anchor base_c cs fid l live def = OK co ->
+             ~ In lbl l ->
+             cs # lbl = Some i ->
+             co # lbl = Some i).
+  { intros. generalize dependent cs.
+    induction l; intros.
+    - simpl in H. inv H. auto.
+    - simpl in H. repeat do_ok. simpl in H0.
+      assert (NOTIN: ~ In lbl l).
+      { unfold not. intros. apply H0. right. auto. }
+      assert (NOTA: a <> lbl).
+      { unfold not. intros. apply H0. left. auto. }
+      specialize (IHl NOTIN c H3). unfold insert_single_anchor in HDO.
+      repeat do_ok. rewrite PTree.gso in IHl; auto.
+      apply IHl. poseq_destr (fresh_sug (Pos.add a spacing) cs) lbl.
+      + erewrite fresh_sug_correct in H1; auto. inv H1.
+      + rewrite PTree.gso; auto. }
+  intros vbase vins fid l_anc lbl live def H0 H1 i H2.
+  unfold anc_insert_version in H0. repeat do_ok.
+  eapply H in HDO; eauto.
+Qed.
+
+
+Ltac rmagreef :=
+  match goal with
+  | [H: eval_expr ?e ?rms = OK ?v,
+        H1: agree ?rms ?rmo ?live |- _] => eapply agree_eval_expr in H; eauto
+  | [H: eval_list ?e ?rms = OK ?v,
+        H1: agree ?rms ?rmo ?live |- _] => eapply agree_eval_list in H; eauto
+  | [H: eval_list_reg ?e ?rms = OK ?v,
+        H1: agree ?rms ?rmo ?live |- _] => eapply agree_eval_list_reg in H; eauto
+  end.
+
+Lemma progress_preserved:
+  forall vbase vins fid l_anc live def s1 s2 p rtl nc i,
+    anc_insert_version vbase fid l_anc live def = OK vins ->
+    find_base_version fid p = Some vbase ->
+    match_states p vbase fid l_anc live def i s1 s2 ->
+    safe (mixed_sem p rtl nc AnchorOn) s1 ->
+    NoDup l_anc ->
+    used l_anc (ver_code vbase) ->
+    (exists r : Integers.Int.int, final_mixed_state (set_version p fid vins) s2 r) \/
+    (exists (t : trace) (s2' : mixed_state),
+        Step (mixed_sem (set_version p fid vins) rtl nc AnchorOn) s2 t s2').
+Proof.
+  intros vbase vins fid l_anc live def s1 s2 p rtl nc i OPTV FINDBASE MATCH SAFE NODUP DEF.
+  inv MATCH.
+  + rewrite OPT in OPTV. inv OPTV.
+    right. exists E0. apply code_anc with (lbl:=lbl)in OPT as CODE; auto.
+    destruct CODE as [freshlbl [rs_def [rs_live [GETDEF [GETLIVE [ANCCODE [BASECODE [i SHIFTCODE]]]]]]]].
+    rewrite GETDEF in DEF0. 
+    exists (Halt_IR (vins, freshlbl, rms), mkmut s' top heap). 
+    assert (exists newrm,
+               update_regmap (identity_varmap (PositiveSet.inter rs_def rs_live)) rms = OK newrm /\
+               agree rms newrm (PositiveSet.inter rs_def rs_live))
+      as [newrm [UPDATE' AGREE]].
+    { eapply defined_deopt_subset_agree; eauto.
+      intros r IN'. apply PositiveSet.inter_spec in IN' as [IN' _]. auto. }
+    eapply Anchor_go_on; eauto.
+  + apply safe_step in SAFE. destruct SAFE as [[t [s'' STEP]]|[r FINAL]].
+    2: { inv FINAL. } 
+    right. rewrite OPT in OPTV. inv OPTV. simpl. inv STEP.
+    * unfold ir_step, ir_int_step in STEP0. repeat sdo_ok.
+      destruct p0. exists t. 
+      { destruct i; repeat sdo_ok.
+          - econstructor. eapply IR_step. unfold ir_step, ir_int_step. rewrite <- SAME_CODE. simpl. eauto.
+          - econstructor. eapply IR_step. unfold ir_step, ir_int_step. rewrite <- SAME_CODE. simpl.
+            unfold fret'. rewrite HDO. simpl. eauto.
+          - poseq_destr f fid.
+            + simpl in HDO. repeat sdo_ok.
+              unfold n_push_interpreter_stackframe in HDO0. simpl in HDO0. destruct top; inv HDO0.
+              econstructor. eapply IR_step. unfold ir_step, ir_int_step. rewrite <- SAME_CODE. simpl.
+              unfold sbind. unfold n_push_interpreter_stackframe. simpl. rewrite HDO. simpl. eauto.
+            + simpl in HDO. repeat sdo_ok.
+              unfold n_push_interpreter_stackframe in HDO0. simpl in HDO0. destruct top; inv HDO0.
+              econstructor. eapply IR_step. unfold ir_step, ir_int_step. rewrite <- SAME_CODE. simpl.
+              unfold sbind. unfold n_push_interpreter_stackframe. simpl. rewrite HDO. simpl. eauto.
+          - destruct (bool_of_int i) eqn:BOOL; repeat sdo_ok.
+            + econstructor. eapply IR_step. unfold ir_step, ir_int_step. rewrite <- SAME_CODE. simpl.
+              rewrite HDO2. simpl. rewrite BOOL. simpl. eauto.
+            + econstructor. eapply IR_step. unfold ir_step, ir_int_step. rewrite <- SAME_CODE. simpl.
+              rewrite HDO2. simpl. rewrite BOOL. simpl. eauto.
+          - econstructor. eapply IR_step. unfold ir_step, ir_int_step. rewrite <- SAME_CODE. simpl.
+            rewrite HDO. simpl. eauto.
+          - econstructor. eapply IR_step. unfold ir_step, ir_int_step. rewrite <- SAME_CODE. simpl.
+            rewrite HDO. simpl. eauto.
+          - econstructor. eapply IR_step. unfold ir_step, ir_int_step. rewrite <- SAME_CODE. simpl.
+            rewrite HDO2. simpl. rewrite HDO. simpl. unfold sbind. unfold n_memset in HDO3.
+            unfold n_memset. destruct (Integers.Int.lt i mem_size). inv HDO3. eauto. inv HDO3.
+          - econstructor. eapply IR_step. unfold ir_step, ir_int_step. rewrite <- SAME_CODE. simpl.
+            rewrite HDO. simpl. unfold sbind. unfold n_memget in HDO2.
+            unfold n_memget. destruct (Integers.Int.lt i mem_size). inv HDO2. 2: inv HDO2.
+            simpl. destruct (heap ! (intpos.pos_of_int i)); inv H0. eauto.
+          - destruct d. repeat sdo_ok. destruct (bool_of_int i) eqn:BOOL; repeat sdo_ok.
+            + econstructor. eapply IR_step. unfold ir_step, ir_int_step. rewrite <- SAME_CODE. simpl.
+              rewrite HDO2. simpl. rewrite BOOL. simpl. eauto.
+            + econstructor. eapply IR_step. unfold ir_step, ir_int_step. rewrite <- SAME_CODE. simpl.
+              rewrite HDO2. simpl. rewrite BOOL. simpl. rewrite HDO. simpl. eauto.
+          - destruct d. repeat sdo_ok. inv HDO. }
+    * exists E0. econstructor. eapply Anchor_go_on; eauto. rewrite <- SAME_CODE. eauto.
+    * exists E0. econstructor. eapply Anchor_deopt; eauto. rewrite <- SAME_CODE. eauto.
+    
+  + rewrite OPT in OPTV. inv OPTV. apply safe_step in SAFE as SAFE'.
+    destruct SAFE' as [[t [s'' STEP]]|[r FINAL]]. 2: { inv FINAL. }
+    specialize (code_notanc vbase vins fid l_anc lbl live def OPT NOTIN).
+    intros SAME_CODE.
+    assert ((ver_code vbase) ! lbl = (ver_code vins) ! lbl) as SAME_CODE'.
+    {
+      destruct ((ver_code vbase) ! lbl) eqn:Hbase.
+      - symmetry. auto.
+      - apply safe_code in SAFE as [i BASE]. rewrite BASE in Hbase. discriminate Hbase.
+    }
+    right. inv STEP.
+    * exists t. unfold ir_step, ir_int_step in STEP0. repeat sdo_ok.
+      { destruct i; repeat sdo_ok.
+          - econstructor. eapply IR_step. unfold ir_step, ir_int_step. rewrite <- SAME_CODE'. simpl. eauto.
+          - econstructor. eapply IR_step. unfold ir_step, ir_int_step. rewrite <- SAME_CODE'. simpl.
+            unfold fret'. rewrite HDO. simpl. eauto.
+          - poseq_destr f fid.
+            + simpl in HDO. repeat sdo_ok.
+              unfold n_push_interpreter_stackframe in HDO0. simpl in HDO0. destruct top; inv HDO0.
+              econstructor. eapply IR_step. unfold ir_step, ir_int_step. rewrite <- SAME_CODE'. simpl.
+              unfold sbind. unfold n_push_interpreter_stackframe. simpl. rewrite HDO. simpl. eauto.
+            + simpl in HDO. repeat sdo_ok.
+              unfold n_push_interpreter_stackframe in HDO0. simpl in HDO0. destruct top; inv HDO0.
+              econstructor. eapply IR_step. unfold ir_step, ir_int_step. rewrite <- SAME_CODE'. simpl.
+              unfold sbind. unfold n_push_interpreter_stackframe. simpl. rewrite HDO. simpl. eauto.
+          - destruct (bool_of_int i) eqn:BOOL; repeat sdo_ok.
+            + econstructor. eapply IR_step. unfold ir_step, ir_int_step. rewrite <- SAME_CODE'. simpl.
+              rewrite HDO2. simpl. rewrite BOOL. simpl. eauto.
+            + econstructor. eapply IR_step. unfold ir_step, ir_int_step. rewrite <- SAME_CODE'. simpl.
+              rewrite HDO2. simpl. rewrite BOOL. simpl. eauto.
+          - econstructor. eapply IR_step. unfold ir_step, ir_int_step. rewrite <- SAME_CODE'. simpl.
+            rewrite HDO. simpl. eauto.
+          - econstructor. eapply IR_step. unfold ir_step, ir_int_step. rewrite <- SAME_CODE'. simpl.
+            rewrite HDO. simpl. eauto.
+          - econstructor. eapply IR_step. unfold ir_step, ir_int_step. rewrite <- SAME_CODE'. simpl.
+            rewrite HDO2. simpl. rewrite HDO. simpl. unfold sbind. unfold n_memset in HDO3.
+            unfold n_memset. destruct (Integers.Int.lt i mem_size). inv HDO3. eauto. inv HDO3.
+          - econstructor. eapply IR_step. unfold ir_step, ir_int_step. rewrite <- SAME_CODE'. simpl.
+            rewrite HDO. simpl. unfold sbind. unfold n_memget in HDO2.
+            unfold n_memget. destruct (Integers.Int.lt i mem_size). inv HDO2. 2: inv HDO2.
+            simpl. destruct (heap ! (intpos.pos_of_int i)); inv H0. eauto.
+          - destruct d. repeat sdo_ok. destruct (bool_of_int i) eqn:BOOL; repeat sdo_ok.
+            + econstructor. eapply IR_step. unfold ir_step, ir_int_step. rewrite <- SAME_CODE'. simpl.
+              rewrite HDO2. simpl. rewrite BOOL. simpl. eauto.
+            + econstructor. eapply IR_step. unfold ir_step, ir_int_step. rewrite <- SAME_CODE'. simpl.
+              rewrite HDO2. simpl. rewrite BOOL. simpl. rewrite HDO. simpl. eauto.
+          - destruct d. repeat sdo_ok. inv HDO. }
+    * exists E0. econstructor. eapply Anchor_go_on; eauto. 
+    * exists E0. econstructor. eapply Anchor_deopt; eauto. 
+
+  + rename s into stk. rename s' into stk'.
+{ apply safe_step in SAFE. destruct SAFE as [[t [s'' STEP]]| [r FINAL]].
+    2: { inv FINAL. left. exists r. constructor. }
+    right. inv STEP.
+    + destruct ms1. eapply addstk_same in STEP0 as [s [APP SAME]]; eauto.
+      2: apply addstk_irstep.
+      exists t. econstructor. eapply IR_step. simpl. eauto.
+    + destruct ms1. eapply addstk_same in STEP0 as [s [APP SAME]]; eauto.
+      2: apply addstk_asmstep.
+      exists t. econstructor. eapply x86_step. simpl. eauto.
+    + econstructor. econstructor. eapply rtl_step; eauto.
+    + destruct ms'. eapply addstk_same in BLOCK as [s [APP SAME]]; eauto.
+      2: { unfold block_step. repeat addstk_auto. unfold exec_block_instr. repeat addstk_auto.
+           unfold ASMinterpreter.prim_sem_dec. repeat addstk_auto. }
+      exists t. econstructor. eapply rtl_block_step. eauto.
+    + destruct ms2, ms3. eapply addstk_same in CALLEE as [s [APP SAME]]; eauto.
+      2: apply addstk_callee.
+      eapply addstk_prim_same in NOT_COMPILED as [stk2 [APP2 SAME2]]; try constructor.
+      apply app_same in APP2. subst.
+      eapply addstk_same in ARGS as [s3 [APP3 SAME3]]; eauto.
+      2: apply addstk_get_args.
+      poseq_destr fid fid0.
+      * econstructor. econstructor.
+        eapply Call_IR with (func:=set_version_function vins func) (ver:=vins); eauto.
+        unfold set_version, set_version_funlist. simpl. rewrite GETF. rewrite PTree.gss. auto.
+      * econstructor. econstructor.
+        eapply Call_IR; eauto. unfold set_version, set_version_funlist. simpl.
+        unfold find_base_version, find_function_ir in FINDBASE.
+        destruct ((prog_funlist p)#fid); inv FINDBASE. rewrite PTree.gso; auto.
+    + destruct ms2, ms3, ms4. eapply addstk_same in CALLEE as [s [APP SAME]]; eauto.
+      2: apply addstk_callee.
+      eapply addstk_prim_same in COMPILED as [stk2 [APP2 SAME2]]; try constructor.
+      apply app_same in APP2. subst.
+      eapply addstk_same in ARGS as [stk3 [APP3 SAME3]]. 2: apply addstk_set_args. subst.
+      eapply addstk_prim_same in LOAD as [stk4 [APP4 SAME4]]; try constructor. subst.
+      exists E0. econstructor. eapply Call_x86; eauto.
+    + destruct ms2, ms3. eapply addstk_same in CALLEE as [s [APP SAME]].
+      2: apply addstk_callee.
+      eapply addstk_prim_same in COMPILED as [stk2 [APP2 SAME2]]; try constructor.
+      apply app_same in APP2. subst.
+      eapply addstk_same in ARGS as [stk3 [APP3 SAME3]]. 2: apply addstk_set_args. subst.
+      econstructor. econstructor. eapply Call_RTL; eauto.
+    + destruct ms1, ms2. eapply addstk_same in CALLEE as [s [APP SAME]].
+      2: apply addstk_callee.
+      eapply addstk_prim_same in COMPILED as [stk2 [APP2 SAME2]]; try constructor.
+      apply app_same in APP2. subst.
+      eapply addstk_same in ARGS as [stk3 [APP3 SAME3]]. 2: apply addstk_set_args. subst.
+      econstructor. econstructor. eapply Call_RTL_Block; eauto.
+    + destruct ms1. unfold jit.get_retval in RETVAL. destruct loc eqn:LOC.
+      * destruct top eqn:TOP; inv RETVAL.
+        simpl in OPEN_SF. unfold n_open_stackframe in OPEN_SF. simpl in OPEN_SF.
+        destruct state_stacktop; inv OPEN_SF.
+        inv MATCHSTACK; inv H0. destruct sf; inv H1.
+        2: { destruct a, p, p0, p. inv H0. }
+        inv MSF.
+        ** econstructor. econstructor. eapply Return_IR; eauto.
+           simpl. unfold sbind. simpl. eauto.
+           simpl. unfold n_open_stackframe. simpl. eauto.
+        ** econstructor. econstructor. eapply Return_IR; eauto.
+           simpl. unfold sbind. simpl. eauto.
+           simpl. unfold n_open_stackframe. simpl. eauto.
+        ** econstructor. econstructor. eapply Return_IR; eauto.
+           simpl. unfold sbind. simpl. eauto.
+           simpl. unfold n_open_stackframe. simpl. eauto.
+      * inv RETVAL.
+        simpl in OPEN_SF. unfold n_open_stackframe in OPEN_SF. simpl in OPEN_SF.
+        destruct state_stacktop; inv OPEN_SF.
+        inv MATCHSTACK; inv H0. destruct sf; inv H1.
+        2: { destruct a, p, p0, p. inv H0. }
+        inv MSF.
+        ** econstructor. econstructor. eapply Return_IR; eauto.
+           simpl. unfold sbind. simpl. eauto.
+           simpl. unfold n_open_stackframe. simpl. eauto.
+        ** econstructor. econstructor. eapply Return_IR; eauto.
+           simpl. unfold sbind. simpl. eauto.
+           simpl. unfold n_open_stackframe. simpl. eauto.
+        ** econstructor. econstructor. eapply Return_IR; eauto.
+           simpl. unfold sbind. simpl. eauto.
+           simpl. unfold n_open_stackframe. simpl. eauto.
+    + destruct loc.
+      * simpl in RETVAL.  repeat sdo_ok.  unfold n_load in HDO. simpl in HDO.
+        destruct top; inv HDO.
+        simpl in OPEN_SF. unfold n_open_stackframe in OPEN_SF. simpl in OPEN_SF.
+        destruct top; inv OPEN_SF. destruct stk; inv H0. destruct s; inv H1.
+        destruct a, p, p0, p. inv H0. inv MATCHSTACK. inv MSF.
+        simpl in SET_RETVAL. unfold n_save in SET_RETVAL. inv SET_RETVAL.
+        simpl in LOAD_CONT. repeat sdo_ok. unfold n_load_prog_code in HDO. simpl in HDO.
+        destruct (nc ! (intpos.pos_of_int caller_fid)) eqn:LOADC; inv HDO.
+        destruct a. simpl in LOAD_CONT.
+        destruct (t ! (intpos.pos_of_int cont_lbl)) eqn:LOAD; inv LOAD_CONT.
+        econstructor. econstructor. eapply Return_x86.
+        ** simpl. unfold sbind. unfold n_load. simpl. eauto.
+        ** simpl. unfold n_open_stackframe. simpl. eauto.
+        ** simpl. unfold n_save. simpl. eauto.
+        ** simpl. unfold sbind. unfold n_load_prog_code. simpl. rewrite LOADC. simpl. rewrite LOAD. eauto.
+        ** eauto.
+      * inv RETVAL. simpl in OPEN_SF. unfold n_open_stackframe in OPEN_SF. simpl in OPEN_SF.
+        destruct top; inv OPEN_SF. destruct stk; inv H0. destruct s; inv H1.
+        destruct a, p, p0, p. inv H0. inv MATCHSTACK. inv MSF.
+        simpl in SET_RETVAL. unfold n_save in SET_RETVAL. inv SET_RETVAL.
+        simpl in LOAD_CONT. repeat sdo_ok. unfold n_load_prog_code in HDO. simpl in HDO.
+        destruct (nc ! (intpos.pos_of_int caller_fid)) eqn:LOADC; inv HDO.
+        destruct a. simpl in LOAD_CONT.
+        destruct (t ! (intpos.pos_of_int cont_lbl)) eqn:LOAD; inv LOAD_CONT.
+        econstructor. econstructor. eapply Return_x86.
+        ** simpl. auto.
+        ** simpl. unfold n_open_stackframe. simpl. eauto.
+        ** simpl. unfold n_save. simpl. eauto.
+        ** simpl. unfold sbind. unfold n_load_prog_code. simpl. rewrite LOADC. simpl. rewrite LOAD. eauto.
+        ** eauto.
+    + destruct loc.
+      * destruct top; inv RETVAL. inv OPEN_SF. unfold n_open_stackframe in H0. simpl in H0.
+        destruct top; inv H0. destruct stk; inv H1. destruct s; inv H0.
+        destruct a, p, p0, p; inv H1. simpl in SETRETVAL. unfold n_save in SETRETVAL. inv SETRETVAL.
+        simpl in NOT_COMPILED. unfold n_check_compiled in NOT_COMPILED. simpl in NOT_COMPILED.
+        destruct (nc ! fid0) eqn:NOT; inv NOT_COMPILED.
+        inv MATCHSTACK. inv MSF.
+        econstructor. econstructor. eapply Return_RTL; eauto.
+        ** simpl. unfold sbind. simpl. eauto.
+        ** simpl. unfold n_open_stackframe. simpl. eauto.
+        ** simpl. unfold n_save. simpl. eauto.
+        ** simpl. unfold n_check_compiled. simpl. rewrite NOT. auto.
+      * inv RETVAL. inv OPEN_SF. unfold n_open_stackframe in H0. simpl in H0.
+        destruct top; inv H0. destruct stk; inv H1. destruct s; inv H0.
+        destruct a, p, p0, p; inv H1. simpl in SETRETVAL. unfold n_save in SETRETVAL. inv SETRETVAL.
+        simpl in NOT_COMPILED. unfold n_check_compiled in NOT_COMPILED. simpl in NOT_COMPILED.
+        destruct (nc ! fid0) eqn:NOT; inv NOT_COMPILED.
+        inv MATCHSTACK. inv MSF.
+        econstructor. econstructor. eapply Return_RTL; simpl; eauto.
+        ** unfold n_open_stackframe. simpl. eauto.
+        ** unfold n_save. simpl. eauto.
+        ** unfold n_check_compiled. simpl. rewrite NOT. auto.
+    + destruct loc.
+      * destruct top; inv RETVAL. inv OPEN_SF. unfold n_open_stackframe in H0. simpl in H0.
+        destruct top; inv H0. destruct stk; inv H1. destruct s; inv H0.
+        destruct a, p, p0, p; inv H1. simpl in SETRETVAL. unfold n_save in SETRETVAL. inv SETRETVAL.
+        simpl in NOT_COMPILED. unfold n_check_compiled in NOT_COMPILED. simpl in NOT_COMPILED.
+        destruct (nc ! fid0) eqn:NOT; inv NOT_COMPILED.
+        inv MATCHSTACK. inv MSF.
+        econstructor. econstructor. eapply Return_RTL_Block; eauto.
+        ** simpl. unfold sbind. simpl. eauto.
+        ** simpl. unfold n_open_stackframe. simpl. eauto.
+        ** simpl. unfold n_save. simpl. eauto.
+        ** simpl. unfold n_check_compiled. simpl. rewrite NOT. auto.
+      * inv RETVAL. inv OPEN_SF. unfold n_open_stackframe in H0. simpl in H0.
+        destruct top; inv H0. destruct stk; inv H1. destruct s; inv H0.
+        destruct a, p, p0, p; inv H1. simpl in SETRETVAL. unfold n_save in SETRETVAL. inv SETRETVAL.
+        simpl in NOT_COMPILED. unfold n_check_compiled in NOT_COMPILED. simpl in NOT_COMPILED.
+        destruct (nc ! fid0) eqn:NOT; inv NOT_COMPILED.
+        inv MATCHSTACK. inv MSF.
+        econstructor. econstructor. eapply Return_RTL_Block; simpl; eauto.
+         ** unfold n_open_stackframe. simpl. eauto.
+         ** unfold n_save. simpl. eauto.
+         ** unfold n_check_compiled. simpl. rewrite NOT. auto.
+    + destruct loc.
+      * destruct top; inv RETVAL. inv OPEN_SF. unfold n_open_stackframe in H0. simpl in H0.
+        destruct top; inv H0. destruct stk; inv H1.
+        2: { destruct s; inv H0. destruct a, p, p0, p; inv H1. }
+        inv MATCHSTACK. econstructor. econstructor. eapply Return_EOE; eauto.
+        simpl. unfold sbind. simpl. eauto.
+        simpl. unfold n_open_stackframe. simpl. eauto.
+      * inv RETVAL. inv OPEN_SF. unfold n_open_stackframe in H0. simpl in H0.
+        destruct top; inv H0. destruct stk; inv H1.
+        2: { destruct s; inv H0. destruct a, p, p0, p; inv H1. }
+        inv MATCHSTACK. econstructor. econstructor. eapply Return_EOE; eauto.
+        simpl. unfold sbind. simpl. eauto.
+        simpl. unfold n_open_stackframe. simpl. eauto.
+    + destruct ms1, ms2. eapply addstk_same in TARGET as [s [APP SAME]].
+      2: apply addstk_target.
+      eapply addstk_same in BUILD_RM as [s2 [APP2 SAME2]].
+      2: apply addstk_build.
+      unfold find_base_version, find_function_ir in FINDBASE.
+      destruct ((prog_funlist p) # ftgt) eqn:FIND; inv FINDBASE. inv FINDF.
+      poseq_destr fid ftgt.
+      * econstructor. econstructor. eapply Deopt; eauto.
+        unfold set_version, set_version_funlist. simpl.
+        rewrite FIND. rewrite PTree.gss; eauto.
+      * econstructor. econstructor. eapply Deopt; eauto.
+        unfold set_version, set_version_funlist. simpl. 
+        destruct ((prog_funlist p) # fid) eqn:FIND'; inv H0. rewrite PTree.gso; eauto.
+      * inv FINDF. 
+    + destruct ms1. eapply addstk_same in PRIM_CALL as [s [APP SAME]].
+      2: { unfold ASMinterpreter.prim_sem_dec. repeat addstk_auto. }
+      econstructor. econstructor. eapply RTL_prim; eauto.
+    + econstructor. econstructor. eapply RTL_end; eauto.
+    + econstructor. econstructor. eapply RTL_block_end; eauto.
+    + econstructor. econstructor. eapply Anchor_go_on; eauto.
+    + econstructor. econstructor. eapply Anchor_deopt; eauto.
+}      
+
+  + right. apply safe_step in SAFE. destruct SAFE as [[t [s'' STEP]]|[r FINAL]].
+    2: { inv FINAL. }
+    inv STEP.
+    * unfold ir_step, ir_int_step in STEP0. repeat sdo_ok.
+      unfold live_dr_transf in AGREE. rewrite HDO1 in AGREE.
+      destruct p0. exists t. 
+      { destruct i; repeat sdo_ok; repeat rmagreef.
+          - econstructor. eapply IR_step. unfold ir_step, ir_int_step. rewrite HDO1. simpl. eauto.
+          - econstructor. eapply IR_step. unfold ir_step, ir_int_step. rewrite HDO1. simpl.
+            unfold fret'. rewrite HDO. simpl. eauto.
+          - poseq_destr f fid.
+            + simpl in HDO. repeat sdo_ok; repeat rmagreef.
+              unfold n_push_interpreter_stackframe in HDO0. simpl in HDO0. destruct top; inv HDO0.
+              econstructor. eapply IR_step. unfold ir_step, ir_int_step. rewrite HDO1. simpl.
+              unfold sbind. rewrite HDO. simpl. eauto.
+            + simpl in HDO. repeat sdo_ok; repeat rmagreef.
+              unfold n_push_interpreter_stackframe in HDO0. simpl in HDO0. destruct top; inv HDO0.
+              econstructor. eapply IR_step. unfold ir_step, ir_int_step. rewrite HDO1. simpl.
+              unfold sbind. unfold n_push_interpreter_stackframe. simpl. rewrite HDO. simpl. eauto.
+          - destruct (bool_of_int i) eqn:BOOL; repeat sdo_ok; repeat rmagreef.
+            + econstructor. eapply IR_step. unfold ir_step, ir_int_step. rewrite HDO1. simpl.
+              eapply agree_eval_reg in HDO2; eauto.
+              rewrite HDO2. simpl. rewrite BOOL. simpl. eauto.
+            + econstructor. eapply IR_step. unfold ir_step, ir_int_step. rewrite HDO1. simpl.
+              eapply agree_eval_reg in HDO2; eauto.
+              rewrite HDO2. simpl. rewrite BOOL. simpl. eauto.
+          - econstructor. eapply IR_step. unfold ir_step, ir_int_step. rewrite HDO1. simpl.
+            rewrite HDO. simpl. eauto.
+          - econstructor. eapply IR_step. unfold ir_step, ir_int_step. rewrite HDO1. simpl.
+            rewrite HDO. simpl. eauto.
+          - econstructor. eapply IR_step. unfold ir_step, ir_int_step. rewrite HDO1. simpl.
+            eapply agree_eval_reg in HDO; eauto. eapply agree_eval_reg in HDO2; eauto.
+            2: { eapply agree_subset; eauto. apply reg_live_subset. }
+            rewrite HDO2. simpl. rewrite HDO. simpl. unfold sbind. unfold n_memset in HDO3.
+            unfold n_memset. destruct (Integers.Int.lt i mem_size). inv HDO3. eauto. inv HDO3.
+          - econstructor. eapply IR_step. unfold ir_step, ir_int_step. rewrite HDO1. simpl.
+            eapply agree_eval_reg in HDO; eauto.
+            rewrite HDO. simpl. unfold sbind. unfold n_memget in HDO2.
+            unfold n_memget. destruct (Integers.Int.lt i mem_size). inv HDO2. 2: inv HDO2.
+            simpl. destruct (heap ! (intpos.pos_of_int i)); inv H0. eauto.
+          - destruct d. repeat sdo_ok. destruct (bool_of_int i) eqn:BOOL; repeat sdo_ok.
+            + econstructor. eapply IR_step. unfold ir_step, ir_int_step. rewrite HDO1. simpl.
+              eapply agree_eval_expr in HDO2; eauto. rewrite HDO2. simpl. rewrite BOOL. simpl. eauto.
+            + econstructor. eapply IR_step. unfold ir_step, ir_int_step. rewrite HDO1. simpl.
+              eapply agree_eval_expr in HDO2; eauto. rewrite HDO2. simpl. rewrite BOOL. simpl.
+              eapply agree_update_regmap in HDO; eauto. rewrite HDO. simpl. eauto.
+              apply agree_sym. eapply agree_subset; eauto. apply expr_live_subset.
+          - destruct d. repeat sdo_ok. inv HDO. }
+    * exists E0. econstructor. eapply Anchor_go_on; eauto. eapply agree_update_regmap in BUILD; eauto.
+      unfold live_dr_transf in AGREE. rewrite ANCHOR in AGREE. apply agree_sym. eauto.
+    * exists E0. econstructor. eapply Anchor_deopt; eauto. eapply agree_update_regmap in BUILD; eauto.
+        unfold live_dr_transf in AGREE. rewrite ANCHOR in AGREE. apply agree_sym. eauto.
+Qed.
+    
+
+Ltac def_ok :=
+  match goal with
+  | [CODE: (ver_code ?vsrc) ! ?lbl = Some ?i |- _] =>
+    eapply def_analyze_correct; eauto; simpl; auto; unfold def_dr_transf; try rewrite CODE; auto
+  end.
+(* WIP *)
+
+Ltac rmagreeb :=
+  match goal with
+  | [ |- agree (?rm1 # ?r <- ?v) (?rm2 # ?r <- ?v) ?rs] => apply agree_insert; auto
+  | [H: eval_expr ?e ?rmo ?v,
+        H1: agree ?rms ?rmo ?rs |- _] => eapply agree_eval_expr in H; apply agree_sym in H1; eauto
+  | [H: eval_list ?e ?rmo ?v,
+        H1: agree ?rms ?rmo ?rs |- _] => eapply agree_eval_list in H; apply agree_sym in H1; eauto
+  | [H: eval_list_expr ?e ?rmo ?v,
+        H1: agree ?rms ?rmo ?rs |- _] => eapply agree_eval_list_expr in H; apply agree_sym in H1; eauto
+  end.
+
+(* The diagram of a backward simulation for lowered steps *)
+(* We only require the same code on both sides, and reuse this lemma for both opt_match and shift_match *)
+Lemma lowered_diagram:
+  forall p vbase fid l_anc live def vins lblsrc lblopt s s' rms ms t s2' f
+         (OPT: anc_insert_version vbase fid l_anc live def = OK vins)
+         (FINDF: find_function fid p = Some f)
+         (NOOPT: fn_opt f = None)
+         (BASE': fn_base f = vbase)
+         (MATCHSTACK: match_stack vbase fid l_anc live def s s')
+         (SAME_CODE: (ver_code vbase) ! lblsrc = (ver_code vins) ! lblopt)
+         (DEFREGS: defined_regs_analysis (ver_code vbase) (fn_params f) (ver_entry vbase) = Some def)
+         (LIVENESS: liveness_analyze vbase = Some live)
+         (DEF: defined rms (def_absstate_get lblsrc def))
+         (STEP: lowered_step (set_version p fid vins) (State s' vins lblopt rms ms) t s2')
+         (SAFE: safe (specir_sem p) (State s vbase lblsrc rms ms)),
+  exists (i: anc_index) (s1': Smallstep.state (specir_sem p)),
+    (SPlus (specir_sem p) (State s vbase lblsrc rms ms) t s1' \/
+     Star (specir_sem p) (State s vbase lblsrc rms ms) t s1' /\ anc_order i Zero) /\
+    match_states p vbase fid l_anc live def i s1' s2'.
+Proof.
+  intros p vbase fid l_anc live def vins lblsrc lblopt s s' rms ms t s2' f OPT FINDF NOOPT BASE' MATCHSTACK SAME_CODE DEFREGS LIVENESS DEF STEP SAFE.
+  assert (BASE: find_base_version fid p = Some vbase).
+  { unfold find_base_version. rewrite FINDF. f_equal. auto. } clear BASE'.
+  inv STEP; rewrite CODE in SAME_CODE.
+  - destruct (in_or_not next l_anc) as [IN | NOTIN].
+    + exists One. exists (State s vbase next rms ms). split.
+      * left. apply plus_one. apply nd_exec_lowered. eapply exec_Nop; eauto.
+      * eapply anc_match; eauto. def_ok. rewrite SAME_CODE. auto.
+    + exists Zero. exists (State s vbase next rms ms). split.
+      * left. apply plus_one. apply nd_exec_lowered. eapply exec_Nop; eauto.
+      * eapply opt_match; eauto. def_ok. rewrite SAME_CODE. auto.
+  - destruct (in_or_not next l_anc) as [IN | NOTIN].
+    + exists One. exists (State s vbase next (rms # reg <- v) ms). split.
+      * left. apply plus_one. apply nd_exec_lowered. eapply exec_Op; eauto.
+      * eapply anc_match; auto. def_ok. rewrite SAME_CODE.
+        apply define_insert. auto.
+    + exists Zero. exists (State s vbase next (rms # reg <- v) ms). split.
+      * left. apply plus_one. apply nd_exec_lowered. eapply exec_Op; eauto.
+      * eapply opt_match; eauto. def_ok. rewrite SAME_CODE.
+        apply define_insert. auto.
+  - destruct (in_or_not next l_anc) as [IN | NOTIN].
+    + exists One. exists (State s vbase next newrm ms). split.
+      * left. apply plus_one. apply nd_exec_lowered. eapply exec_Move; eauto.
+      * eapply anc_match; auto. def_ok. rewrite SAME_CODE.
+        eapply define_insert_list; eauto.
+    + exists Zero. exists (State s vbase next newrm ms). split.
+      * left. apply plus_one. apply nd_exec_lowered. eapply exec_Move; eauto.
+      * eapply opt_match; eauto. def_ok. rewrite SAME_CODE.
+        eapply define_insert_list; eauto.
+  - destruct (in_or_not (pc_cond v iftrue iffalse) l_anc) as [IN | NOTIN].
+    + exists One. exists (State s vbase (pc_cond v iftrue iffalse) rms ms). split.
+      * left. apply plus_one. apply nd_exec_lowered. eapply exec_Cond; eauto.
+      * eapply anc_match; auto. def_ok. destruct v. destruct z; auto. rewrite SAME_CODE. auto.
+    + exists Zero. exists (State s vbase (pc_cond v iftrue iffalse) rms ms). split.
+      * left. apply plus_one. apply nd_exec_lowered. eapply exec_Cond; eauto.
+      * eapply opt_match; auto. def_ok. destruct v. destruct z; auto. rewrite SAME_CODE. auto.
+  - poseq_destr fid fid0.
+    +                           (* calling the optimized function *)
+      assert (ISBASE: vbase = current_version f).
+      { unfold find_base_version in BASE. rewrite FINDF in BASE. inv BASE.
+        unfold current_version. rewrite NOOPT. auto. }
+      assert (ISINS: vins = current_version func).
+      { unfold current_version. eapply find_function_same in FINDF; eauto.
+        rewrite FINDF0 in FINDF. inv FINDF. simpl. auto. }
+      assert (SAME_ENTRY:ver_entry vbase = ver_entry vins).
+      { unfold anc_insert_version in OPT. repeat do_ok. simpl. auto. }
+      assert (SAME_PARAMS: fn_params f = fn_params func).
+      { erewrite find_function_same in FINDF0; eauto. inv FINDF0.
+        unfold set_version_function. auto. }
+      destruct (in_or_not (ver_entry(current_version f)) l_anc) as [IN|NOTIN].
+      * exists One. exists (State (Stackframe retreg vbase next rms :: s) (current_version f) (ver_entry (current_version f)) newrm ms). split.
+        ** left. apply plus_one. apply nd_exec_lowered. eapply exec_Call; eauto.
+           eapply same_params in FINDF0 as PARAMS; eauto. rewrite PARAMS. auto.
+        ** rewrite <- ISBASE. rewrite <- ISINS.
+           rewrite SAME_ENTRY. apply anc_match; auto.
+           *** constructor; auto. constructor; auto.
+               intro. def_ok. rewrite SAME_CODE. apply define_insert. auto.
+           *** rewrite <- SAME_ENTRY. eapply def_analyze_init; eauto.
+               rewrite SAME_PARAMS. eauto.
+           *** rewrite <- ISBASE in IN. rewrite <- SAME_ENTRY. auto.
+      * exists Zero. exists (State (Stackframe retreg vbase next rms :: s) (current_version f) (ver_entry (current_version f)) newrm ms). split.
+        ** left. apply plus_one. apply nd_exec_lowered. eapply exec_Call; eauto.
+           eapply same_params in FINDF0 as PARAMS; eauto. rewrite PARAMS. auto.
+        ** rewrite <- ISBASE. rewrite <- ISINS.
+           rewrite SAME_ENTRY. apply opt_match; auto.
+           *** constructor; auto. constructor; auto.
+               intro. def_ok. rewrite SAME_CODE. apply define_insert. auto.
+           *** rewrite <- SAME_ENTRY. eapply def_analyze_init; eauto.
+               rewrite SAME_PARAMS. eauto.
+           *** rewrite <- ISBASE in NOTIN. rewrite <- SAME_ENTRY. auto.
+    + exists Zero. exists (State (Stackframe retreg vbase next rms :: s) (current_version func) (ver_entry (current_version func)) newrm ms). split.
+      * left. apply plus_one. apply nd_exec_lowered. eapply exec_Call; eauto.
+        erewrite <- find_function_unchanged in FINDF0; auto.
+      * apply refl_match; auto. constructor; auto. constructor; auto.
+        intro. def_ok. rewrite SAME_CODE. apply define_insert. auto.
+  - inv MATCHSTACK. inv MSF.
+    + exists Zero. exists (State s1 fprev next (rmprev # retreg <- retval) ms). split.
+      * left. apply plus_one. apply nd_exec_lowered. eapply exec_Return; eauto.
+      * apply refl_match. auto.
+    + exists Zero. exists (State s1 fprev next (rms0 # retreg <- retval) ms). split.
+      * left. apply plus_one. apply nd_exec_lowered. eapply exec_Return; eauto.
+      * apply deopt_match; auto.
+    + rewrite ANC_INSERT in OPT. inv OPT. (* returning into the optimized version *)
+      destruct (in_or_not next l_anc).
+      * exists One. exists (State s1 vbase next (rmprev#retreg<-retval) ms). split.
+        ** left. apply plus_one. apply nd_exec_lowered. eapply exec_Return; eauto.
+        ** eapply anc_match; eauto.
+      * exists Zero. exists (State s1 vbase next (rmprev#retreg<-retval) ms). split.
+        ** left. apply plus_one. apply nd_exec_lowered. eapply exec_Return; eauto.
+        ** eapply opt_match; eauto.
+  - inv MATCHSTACK. exists One. exists (Final retval ms). split.
+    * left. apply plus_one. apply nd_exec_lowered. eapply exec_Return_Final; eauto.
+    * eapply final_match; eauto.
+  - destruct (in_or_not next l_anc) as [IN | NOTIN].
+    + exists One. exists (State s vbase next rms ms). split.
+      * left. apply plus_one. apply nd_exec_lowered. eapply exec_Printexpr; eauto.
+      * eapply anc_match; auto. def_ok. rewrite SAME_CODE. auto.
+    + exists Zero. exists (State s vbase next rms ms). split.
+      * left. apply plus_one. apply nd_exec_lowered. eapply exec_Printexpr; eauto.
+      * eapply opt_match; eauto. def_ok. rewrite SAME_CODE. auto.
+  - destruct (in_or_not next l_anc) as [IN | NOTIN].
+    + exists One. exists (State s vbase next rms ms). split.
+      * left. apply plus_one. apply nd_exec_lowered. eapply exec_Printstring; eauto.
+      * eapply anc_match; auto. def_ok. rewrite SAME_CODE. auto.
+    + exists Zero. exists (State s vbase next rms ms). split.
+      * left. apply plus_one. apply nd_exec_lowered. eapply exec_Printstring; eauto.
+      * eapply opt_match; eauto. def_ok. rewrite SAME_CODE. auto.
+  - destruct (in_or_not next l_anc) as [IN | NOTIN].
+    + exists One. exists (State s vbase next rms newms). split.
+      * left. apply plus_one. apply nd_exec_lowered. eapply exec_Store; eauto.
+      * eapply anc_match; auto. def_ok. rewrite SAME_CODE. auto.
+    + exists Zero. exists (State s vbase next rms newms). split.
+      * left. apply plus_one. apply nd_exec_lowered. eapply exec_Store; eauto.
+      * eapply opt_match; eauto. def_ok. rewrite SAME_CODE. auto.
+  - destruct (in_or_not next l_anc) as [IN | NOTIN].
+    + exists One. exists (State s vbase next (rms#reg<-val) ms). split.
+      * left. apply plus_one. apply nd_exec_lowered. eapply exec_Load; eauto.
+      * eapply anc_match; eauto. def_ok. rewrite SAME_CODE.
+        apply define_insert. auto.
+    + exists Zero. exists (State s vbase next (rms#reg<-val) ms). split.
+      * left. apply plus_one. apply nd_exec_lowered. eapply exec_Load; eauto.
+      * eapply opt_match; eauto. def_ok. rewrite SAME_CODE. apply define_insert. auto.
+  - destruct (in_or_not next l_anc) as [IN | NOTIN].
+    + exists One. exists (State s vbase next rms ms). split.
+      * left. apply plus_one. apply nd_exec_lowered. eapply exec_Assume_holds; eauto.
+      * eapply anc_match; auto. def_ok. rewrite SAME_CODE. auto.
+    + exists Zero. exists (State s vbase next rms ms). split.
+      * left. apply plus_one. apply nd_exec_lowered. eapply exec_Assume_holds; eauto.
+      * eapply opt_match; auto. def_ok. rewrite SAME_CODE. auto.
+  - apply <- synth_frame_unchanged in SYNTH. exists Zero.
+    rewrite <- base_version_unchanged in FINDF0.
+    exists (State (synth ++ s) newver la newrm ms). split.
+    + left. apply plus_one. apply nd_exec_lowered. eapply exec_Assume_fails; eauto.
+    + apply refl_match. apply match_app. auto.
+Qed.
+
+(* Proved directly with a backward simulation *)
+Theorem anchor_insertion_correct:
+  forall p fid lbllist newp,
+    insert_anchor fid lbllist p = OK newp ->
+    backward_internal_simulation p newp.
+Proof.
+  intros p fid lbllist newp OPT. unfold insert_anchor in OPT. repeat do_ok.
+  rename HDO1 into FINDOPTF. rename d into def. rename l into live.
+  set (l_anc := (clean_label_list def (ver_code (fn_base f)) lbllist)).
+  rename v into vins. unfold check_no_opt in HDO0. destruct (fn_opt f) eqn:NO_OPT; inv HDO0.
+  set (vbase := (fn_base f)). fold l_anc vbase in HDO2. rename v0 into vins.
+  assert (OPTV: anc_insert_version vbase fid l_anc live def = OK vins) by auto.
+  unfold anc_insert_version in HDO3. repeat do_ok.
+  set (vins := {|ver_code := c; ver_entry := ver_entry vbase |}). fold vins in OPTV.
+  apply Backward_internal_simulation with (bsim_order := anc_order) (bsim_match_states := match_states p vbase fid l_anc live def).
+  - apply wfounded.
+  - apply trans.
+
+  - unfold reflexive_forge. intros synchro stack r1 s1 ms FORGE.
+    destruct synchro; simpl in FORGE; repeat do_ok; simpl.
+    + poseq_destr f0 fid.  (* is the called function the optimized one? *)
+      * erewrite find_function_same; eauto. simpl. rewrite HDO1. simpl.
+        rewrite FINDOPTF in HDO3. inv HDO3.
+        assert (CURRENT:  vbase  = (current_version f1)).
+        { unfold vbase. unfold current_version. rewrite NO_OPT. auto. }
+        rewrite <- CURRENT.
+        { destruct (in_or_not (ver_entry(current_version f1)) l_anc) as [IN|NOTIN]; repeat (esplit; eauto).
+          - unfold vbase. eapply anc_match; eauto.
+            + apply match_stack_same.
+            + unfold clean_label_list in l_anc.
+              apply interpreter_proof.init_regs_correct in HDO1.
+              eapply def_analyze_init; eauto.
+            + rewrite <- CURRENT in IN. unfold vbase in IN. auto.
+          - eapply opt_match.
+            + apply match_stack_same.
+            + apply interpreter_proof.init_regs_correct in HDO1.
+              eapply def_analyze_init; eauto.
+            + auto.
+            + rewrite <- CURRENT in NOTIN. auto.  }
+      * erewrite <- find_function_unchanged; eauto. rewrite HDO3. simpl. rewrite HDO1. simpl.
+        repeat (esplit; eauto). econstructor. apply match_stack_same.
+    + destruct stack; try destruct s; inv FORGE.
+      * repeat (esplit; eauto). constructor.
+      * repeat (esplit; eauto). simpl. econstructor. apply match_stack_same.
+    + destruct d. repeat do_ok. simpl. rewrite <- base_version_unchanged. rewrite HDO1. simpl.
+      repeat (esplit; eauto). simpl. econstructor. apply match_stack_same.
+    + inv FORGE. destruct r1; repeat (esplit; eauto).
+      * simpl. eapply refl_match. apply match_stack_same.
+      * simpl. eapply final_match.
+
+  - intros i s1 s2 r MATCH SAFE FINAL. inv FINAL. inv MATCH. exists (Final r ms). split.
+    apply star_refl. constructor.
+
+  - intros. eapply progress_preserved; eauto. unfold find_base_version. rewrite FINDOPTF. eauto.
+    apply nodup_clean. apply used_clean.
+
+  - intros s2 t s2' STEP i s1 MATCH SAFE.
+    assert (NODUP: NoDup l_anc) by apply nodup_clean.
+    assert (DEF: used l_anc (ver_code vbase)) by apply used_clean.
+    inv MATCH.
+
+    + rewrite OPT in OPTV. inv OPTV. (* anc_match *)
+      eapply code_anc in IN as [fresh [rs_def [rs_live [GETDEF [GETLIVE [ANCCODE [FRESH [nextinstr [CODESRC CODEOPT]]]]]]]]]; eauto.
+      inv STEP.
+      { inv STEP0; rewrite CODE in ANCCODE; inv ANCCODE. }
+      { exists Zero. exists (State s vbase lbl rms ms). split. (* stuttering, ANC goes on  *)
+        - right. split. 2:constructor. apply star_refl.
+        - inv DEOPT_COND. rewrite CODE in ANCCODE. inv ANCCODE. inv SYNTH. eapply shift_match; auto.
+          unfold not; intros. apply DEF in H as [i CODE']. rewrite CODE' in FRESH. inv FRESH.
+          rewrite CODESRC. rewrite CODEOPT. auto. }
+      { exists Zero. exists (State s vbase lbl rms ms). split. (* stuttering, ANC deoptimizes *)
+        - right. split. 2:constructor. apply star_refl.
+        - inv DEOPT_COND. rewrite CODE in ANCCODE. inv ANCCODE. inv SYNTH. simpl.
+          assert (BASE: vbase = newver).
+          { simpl in FINDF. rewrite <- base_version_unchanged in FINDF. unfold find_base_version in FINDF.
+            rewrite FINDOPTF in FINDF. inv FINDF. unfold vbase. auto. }
+          rewrite <- BASE. eapply deopt_match; eauto.
+          rewrite GETDEF in DEF0.
+          eapply defined_deopt_subset_agree in DEF0 as DEF0'; eauto.
+          2: { intros r IN. apply IN. }        
+          destruct DEF0' as [rmdeopt [UPDATE' AGREE]].
+          eapply deopt_subset_agree in UPDATE as AGREE'; eauto.
+          2: { intros r IN. apply PositiveSet.inter_spec in IN as [IN _]. auto. }
+          intros r IN.
+          destruct (PositiveSet.mem r rs_def) eqn:Emem.
+          + apply AGREE'. apply PositiveSet.inter_spec. split; auto.
+          + assert (rms ! r = None).
+            { unfold defined in DEF0. specialize (DEF0 r).
+              rewrite <- PositiveSet.mem_spec in DEF0.
+              rewrite Emem in DEF0. destruct (rms ! r) eqn:Er; auto.
+              assert (exists v0, Some v = Some v0).
+              { exists v. auto. }
+              apply DEF0 in H. discriminate. }
+            rewrite H. symmetry. eapply update_not_captured; eauto.
+            intros IN'. apply PositiveSet.inter_spec in IN' as [IN' _].
+            rewrite <- PositiveSet.mem_spec in IN'.
+            rewrite IN' in Emem. discriminate. }
+    + rewrite OPT in OPTV. inv OPTV. (* shift_match *)
+      inv STEP.
+      { eapply lowered_diagram; eauto. }
+      * inv DEOPT_COND.         (* Anchor steps can't happen in shift_match *)
+        rewrite CODE in SAME_CODE. unfold vbase in SAME_CODE. apply (base_no_spec f) in SAME_CODE.
+        exfalso. apply SAME_CODE. constructor.
+      * inv DEOPT_COND.         (* Anchor steps can't happen in shift_match *)
+        rewrite CODE in SAME_CODE. unfold vbase in SAME_CODE. apply (base_no_spec f) in SAME_CODE.
+        exfalso. apply SAME_CODE. constructor.
+
+    + rewrite OPT in OPTV. inv OPTV. (* opt_match *)
+      eapply code_preservation in NOTIN as SAME_CODE; eauto.
+      inv STEP.
+      { eapply lowered_diagram; eauto. }
+      * inv DEOPT_COND. (* Anchor steps can't happen in opt_match *)
+        rewrite CODE in SAME_CODE. unfold vbase in SAME_CODE. apply (base_no_spec f) in SAME_CODE.
+        exfalso. apply SAME_CODE. constructor.
+      * inv DEOPT_COND. (* Anchor steps can't happen in opt_match *)
+        rewrite CODE in SAME_CODE. unfold vbase in SAME_CODE. apply (base_no_spec f) in SAME_CODE.
+        exfalso. apply SAME_CODE. constructor.
+
+    + inv STEP.                 (* refl_match *)
+      { inv STEP0.
+        - exists Zero. exists (State s v' next rms ms). split.
+          + left. apply plus_one. apply nd_exec_lowered. eapply exec_Nop; eauto.
+          + eapply refl_match; eauto.
+        - exists Zero. exists (State s v' next (rms#reg<-v) ms). split.
+          + left. apply plus_one. apply nd_exec_lowered. eapply exec_Op; eauto.
+          + apply refl_match; auto.
+        - exists Zero. exists (State s v' next newrm ms). split.
+          + left. apply plus_one. apply nd_exec_lowered. eapply exec_Move; eauto.
+          + apply refl_match; auto.
+        - exists Zero. exists (State s v' (pc_cond v iftrue iffalse) rms ms). split.
+          + left. apply plus_one. apply nd_exec_lowered. eapply exec_Cond; eauto.
+          + apply refl_match; auto.
+        - poseq_destr fid0 fid.
+          + destruct (in_or_not (ver_entry vbase) l_anc) as [IN|NOTIN].
+            * exists One. exists (State (Stackframe retreg v' next rms ::s) (current_version f) (ver_entry (current_version f)) newrm ms). split.
+              ** left. apply plus_one. apply nd_exec_lowered. eapply exec_Call; eauto.
+                 simpl in FINDF. eapply same_params in FINDOPTF; eauto.
+                 rewrite FINDOPTF. auto.
+              ** simpl in FINDF. erewrite find_function_same in FINDF; eauto. inv FINDF.
+                 unfold current_version. rewrite NO_OPT. simpl.
+                 apply anc_match; auto.
+                 2: { eapply def_analyze_init; eauto. }
+                 constructor; auto. eapply frame_same; eauto.
+            * exists Zero. exists (State (Stackframe retreg v' next rms ::s) (current_version f) (ver_entry (current_version f)) newrm ms). split.
+              ** left. apply plus_one. apply nd_exec_lowered. eapply exec_Call; eauto.
+                 simpl in FINDF. eapply same_params in FINDOPTF; eauto.
+                 rewrite FINDOPTF. auto.
+              ** simpl in FINDF. erewrite find_function_same in FINDF; eauto. inv FINDF.
+                 unfold current_version. rewrite NO_OPT. simpl.
+                 apply opt_match; auto.
+                 2: { eapply def_analyze_init; eauto. }
+                 constructor; auto. constructor. 
+          + simpl in FINDF. rewrite <- find_function_unchanged in FINDF; auto.
+            exists Zero. exists (State (Stackframe retreg v' next rms :: s) (current_version func) (ver_entry (current_version func)) newrm ms). split.
+            * left. apply plus_one. apply nd_exec_lowered. eapply exec_Call; eauto.
+            * apply refl_match; auto. constructor; auto. constructor.
+        - inv MATCHSTACK. inv MSF.
+          + exists Zero. exists (State s1 fprev next (rmprev#retreg<-retval) ms). split.
+            * left. apply plus_one. apply nd_exec_lowered. eapply exec_Return; eauto.
+            * apply refl_match; auto.
+          + exists Zero. exists (State s1 vbase next (rms0#retreg<-retval) ms). split.
+            * left. apply plus_one. apply nd_exec_lowered. eapply exec_Return; eauto.
+            * apply deopt_match; auto.
+          + destruct (in_or_not next l_anc).
+            * exists One. exists (State s1 vbase next (rmprev#retreg<-retval) ms). split.
+              ** left. apply plus_one. apply nd_exec_lowered. eapply exec_Return; eauto.
+              ** apply anc_match; auto.
+            * exists Zero. exists (State s1 vbase next (rmprev#retreg<-retval) ms). split.
+              ** left. apply plus_one. apply nd_exec_lowered. eapply exec_Return; eauto.
+              ** apply opt_match; auto.
+        - inv MATCHSTACK. exists One. exists (Final retval ms). split.
+          + left. apply plus_one. apply nd_exec_lowered. eapply exec_Return_Final; eauto.
+          + apply final_match; auto.
+        - exists Zero. exists (State s v' next rms ms). split.
+          + left. apply plus_one. apply nd_exec_lowered. eapply exec_Printexpr; eauto.
+          + apply refl_match; auto.
+        - exists Zero. exists (State s v' next rms ms). split.
+          + left. apply plus_one. apply nd_exec_lowered. eapply exec_Printstring; eauto.
+          + apply refl_match; auto.
+        - exists Zero. exists (State s v' next rms newms). split.
+          + left. apply plus_one. apply nd_exec_lowered. eapply exec_Store; eauto.
+          + apply refl_match; auto.
+        - exists Zero. exists (State s v' next (rms#reg<-val) ms). split.
+          + left. apply plus_one. apply nd_exec_lowered. eapply exec_Load; eauto.
+          + apply refl_match; auto.
+        - exists Zero. exists (State s v' next rms ms). split.
+          + left. apply plus_one. apply nd_exec_lowered. eapply exec_Assume_holds; eauto.
+          + apply refl_match; auto.
+        - exists Zero. exists (State (synth++s) newver la newrm ms). split.
+          + left. apply plus_one. apply nd_exec_lowered. eapply exec_Assume_fails; eauto.
+            erewrite base_version_unchanged; eauto.
+            * apply FINDF.
+            * apply synth_frame_unchanged in SYNTH. apply SYNTH.
+          + apply refl_match; auto. apply match_app; auto. }
+      * inv DEOPT_COND. simpl in FINDF. rewrite <- base_version_unchanged in FINDF.
+        apply synth_frame_unchanged in SYNTH.
+        exists Zero. exists (State s v' next rms ms). split.
+        left. apply plus_one. eapply nd_exec_Anchor_go_on.
+        econstructor; eauto. apply refl_match; auto.
+      * inv DEOPT_COND. simpl in FINDF. rewrite <- base_version_unchanged in FINDF.
+        apply synth_frame_unchanged in SYNTH.
+        exists Zero. exists (State (synth ++ s) newver la newrm ms). split.
+        left. apply plus_one. eapply nd_exec_Anchor_deopt.
+        econstructor; eauto. apply refl_match; auto. apply match_app; auto.
+
+    + inv STEP.                (* deopt_match *)
+      { inv STEP0; unfold live_dr_transf in AGREE; rewrite CODE in AGREE.
+        - exists Zero. exists (State s vbase next rms ms). split.
+          + left. apply plus_one. apply nd_exec_lowered. eapply exec_Nop; eauto.
+          + apply deopt_match; auto.            
+            eapply agree_transfer; eauto. simpl. left. auto.
+        - exists Zero. exists (State s vbase next (rms#reg<-v) ms). split.
+          + left. apply plus_one. apply nd_exec_lowered.
+            eapply exec_Op; eauto. rmagreeb.
+          + apply deopt_match; auto. eapply agree_transfer; eauto.
+            2: { apply agree_insert_dead. eapply expr_live_agree. eauto. }
+            simpl. left. auto.
+        - eapply agree_update_movelist in UPDATE as UPDATE'; eauto.
+          destruct UPDATE' as [rm1u [UPDATE' NEXT]]; eauto.
+          exists Zero. exists (State s vbase next rm1u ms). split.
+          + left. apply plus_one. apply nd_exec_lowered. eapply exec_Move; eauto.
+          + apply deopt_match; auto. eapply agree_transfer; eauto.
+            2: { apply agree_movelist_dead with (ml := ml) (rms := rms) (rmo := rmo); auto. }
+            simpl. left. auto.         
+        - exists Zero. exists (State s vbase (pc_cond v iftrue iffalse) rms ms). split.
+          + left. apply plus_one. apply nd_exec_lowered.
+            eapply exec_Cond; eauto. rmagreeb.
+          + apply deopt_match; auto. eapply agree_transfer; eauto.
+            2: { eapply expr_live_agree. eauto. }
+            simpl. destruct v; destruct z; simpl;
+                     try (left; reflexivity); try (right; reflexivity);
+                       try (right; left; reflexivity).
+        - poseq_destr fid0 fid.
+          + destruct (in_or_not (ver_entry vbase) l_anc) as [IN|NOTIN].
+            * exists One. exists (State (Stackframe retreg vbase next rms ::s) (current_version f) (ver_entry (current_version f)) newrm ms). split.
+              ** left. apply plus_one. apply nd_exec_lowered.
+                 eapply exec_Call; eauto. rmagreeb.
+                 simpl in FINDF. eapply same_params in FINDOPTF; eauto.
+                 rewrite FINDOPTF. auto.
+              ** simpl in FINDF. erewrite find_function_same in FINDF; eauto. inv FINDF.
+                 unfold current_version. rewrite NO_OPT. simpl.
+                 apply anc_match; auto.
+                 2: { eapply def_analyze_init; eauto. }
+                 constructor; auto. eapply frame_deopt; eauto.
+                 intros. eapply agree_transfer; eauto. 
+                 2: { apply agree_insert_dead.
+                      eapply expr_list_live_agree. eauto. }
+                 simpl. left. auto.
+            * exists Zero. exists (State (Stackframe retreg vbase next rms ::s) (current_version f) (ver_entry (current_version f)) newrm ms). split.
+              ** left. apply plus_one. apply nd_exec_lowered.
+                 eapply exec_Call; eauto. rmagreeb.
+                 simpl in FINDF. eapply same_params in FINDOPTF; eauto.
+                 rewrite FINDOPTF. auto.
+              ** simpl in FINDF. erewrite find_function_same in FINDF; eauto. inv FINDF.
+                 unfold current_version. rewrite NO_OPT. simpl.
+                 apply opt_match; auto.
+                 2: { eapply def_analyze_init; eauto. }
+                 constructor; auto. constructor.
+                 intros. eapply agree_transfer; eauto. 
+                 2: { apply agree_insert_dead.
+                      eapply expr_list_live_agree. eauto. }
+                 simpl. left. auto.
+          + simpl in FINDF. rewrite <- find_function_unchanged in FINDF; auto. exists Zero.
+            exists (State (Stackframe retreg vbase next rms :: s) (current_version func) (ver_entry (current_version func)) newrm ms). split.
+            * left. apply plus_one. apply nd_exec_lowered.
+              eapply exec_Call; eauto. rmagreeb.
+            * apply refl_match; auto. constructor; auto. constructor.
+              intros. eapply agree_transfer; eauto. 
+              2: { apply agree_insert_dead.
+                   eapply expr_list_live_agree. eauto. }
+              simpl. left. auto.
+        - inv MATCHSTACK. inv MSF.
+          + exists Zero. exists (State s1 fprev next (rmprev#retreg<-retval) ms). split.
+            * left. apply plus_one. apply nd_exec_lowered.
+              eapply exec_Return; eauto. rmagreeb.
+            * apply refl_match; auto.
+          + exists Zero. exists (State s1 vbase next (rms0#retreg<-retval) ms). split.
+            * left. apply plus_one. apply nd_exec_lowered.
+              eapply exec_Return; eauto. rmagreeb.
+            * apply deopt_match; auto. 
+          + destruct (in_or_not next l_anc).
+            * exists One. exists (State s1 vbase next (rmprev#retreg<-retval) ms). split.
+              ** left. apply plus_one. apply nd_exec_lowered.
+                 eapply exec_Return; eauto. rmagreeb.
+              ** apply anc_match; auto. 
+            * exists Zero. exists (State s1 vbase next (rmprev#retreg<-retval) ms). split.
+              ** left. apply plus_one. apply nd_exec_lowered.
+                 eapply exec_Return; eauto. rmagreeb.
+              ** apply opt_match; auto. 
+        - inv MATCHSTACK. exists One. exists (Final retval ms). split.
+          + left. apply plus_one. apply nd_exec_lowered.
+            eapply exec_Return_Final; eauto. rmagreeb.
+          + apply final_match; auto.
+        - exists Zero. exists (State s vbase next rms ms). split.
+          + left. apply plus_one. apply nd_exec_lowered.
+            eapply exec_Printexpr; eauto. rmagreeb.
+          + apply deopt_match; auto. eapply agree_transfer; eauto.
+            2: { eapply expr_live_agree. eauto. }
+            simpl. left. auto.
+        - exists Zero. exists (State s vbase next rms ms). split.
+          + left. apply plus_one. apply nd_exec_lowered. eapply exec_Printstring; eauto.
+          + apply deopt_match; auto.
+            eapply agree_transfer; eauto. simpl. left. auto.
+        - exists Zero. exists (State s vbase next rms newms). split.
+          + left. apply plus_one. apply nd_exec_lowered. eapply exec_Store; eauto.
+            * clear EVAL_AD. rmagreeb.
+            * clear EVAL_ST. rmagreeb.
+              eapply expr_live_agree. eauto.
+          + apply deopt_match; auto. eapply agree_transfer; eauto.
+            simpl. left. auto.
+            repeat (eapply expr_live_agree; eauto).
+        - exists Zero. exists (State s vbase next (rms#reg<-val) ms). split.
+          + left. apply plus_one. apply nd_exec_lowered.
+            eapply exec_Load; eauto. rmagreeb.
+          + apply deopt_match; auto. eapply agree_transfer; eauto. 
+            2: { apply agree_insert_dead.
+                 eapply expr_live_agree. eauto. }
+            simpl. left. auto.
+        - exists Zero. exists (State s vbase next rms ms). split.
+          + left. apply plus_one. apply nd_exec_lowered. destruct tgt.
+            eapply exec_Assume_holds; eauto. rmagreeb.
+          + apply deopt_match; auto. eapply agree_transfer; eauto.
+            2: { destruct tgt.
+                 eapply synth_live_agree. eapply varmap_live_agree.
+                 eapply expr_list_live_agree. eauto. }
+            simpl. left. auto.
+        - eapply agree_update_regmap in UPDATE; eauto.
+          2: { eapply expr_list_live_agree. eauto. }
+          eapply agree_synthesize_frame in SYNTH; eauto.
+          2: { eapply varmap_live_agree. eapply expr_list_live_agree. eauto. }
+          exists Zero. exists (State (synth++s) newver la newrm ms). split.
+          + left. apply plus_one. apply nd_exec_lowered.
+            eapply exec_Assume_fails; eauto; try rmagreeb.
+            * erewrite base_version_unchanged; eauto. apply FINDF.
+            * apply synth_frame_unchanged in SYNTH. eauto.
+          + apply refl_match; auto. apply match_app; auto. }
+      * inv DEOPT_COND. simpl in FINDF.
+        rewrite <- base_version_unchanged in FINDF.
+        unfold live_dr_transf in AGREE. rewrite CODE in AGREE.
+        apply synth_frame_unchanged in SYNTH.
+        eapply agree_update_regmap in UPDATE; eauto.
+        eapply agree_synthesize_frame in SYNTH; eauto.
+        2: { eapply varmap_live_agree. eauto. }
+        exists Zero. exists (State s vbase next rms ms). split.
+        ** left. apply plus_one. eapply nd_exec_Anchor_go_on.
+           econstructor; eauto.
+        ** apply deopt_match; auto.
+           eapply agree_transfer; eauto. 
+           2: { eapply synth_live_agree. eapply varmap_live_agree. eauto. }
+           simpl. left. auto.
+      * inv DEOPT_COND. simpl in FINDF.
+        rewrite <- base_version_unchanged in FINDF.
+        unfold live_dr_transf in AGREE. rewrite CODE in AGREE.
+        apply synth_frame_unchanged in SYNTH.
+        eapply agree_update_regmap in UPDATE; eauto.
+        eapply agree_synthesize_frame in SYNTH; eauto.
+        2: { eapply varmap_live_agree. eauto. }
+        exists Zero. exists (State (synth ++ s) newver la newrm ms). split.
+        ** left. apply plus_one. eapply nd_exec_Anchor_deopt.
+           econstructor; eauto.
+        ** apply refl_match; auto. apply match_app; auto. 
+
+    + inv STEP. inv STEP0.      (* final_match *)
+Qed.
